cfrontend/ChkCgenproof.v
@@ -17,454 +17,455 @@ Require Import Coqlib Maps Errors Integers.
 Require Import AST Linking.
 Require Import Values Memory Events Globalenvs Smallstep.
 Require Import Ctypes ChkCtypes Cop ChkCop ChkCsyntax Csyntax ChkCsem Csem ChkCstrategy Cstrategy.
-Require Import ChkCgen ChkCgenspec.
+Require Import ChkCgen.
 
 (** ** Relational specification of the translation. *)
 
-Definition match_prog (p: ChkCsyntax.program) (tp: Csyntax.program) :=
-  match_program (fun ctx f tf => tr_fundef f tf) eq p tp
-  /\ prog_types tp = prog_types p.
+(* Definition match_prog (p: ChkCsyntax.program) (tp: Csyntax.program) := *)
+(*   match_program (fun ctx f tf => tr_fundef f tf) eq p tp *)
+(*   /\ prog_types tp = prog_types p. *)
 
-Lemma transf_program_match:
-  forall p tp, transl_program p = OK tp -> match_prog p tp.
-Proof.
-  unfold transl_program; intros. monadInv H. split; auto.
-  unfold program_of_program; simpl. destruct x; simpl.
-  eapply match_transform_partial_program_contextual. eexact EQ.
-  intros. apply transl_fundef_spec; auto.
-Qed.
+(* Lemma transf_program_match: *)
+(*   forall p tp, transl_program p = OK tp -> match_prog p tp. *)
+(* Proof. *)
+(* (*   unfold transl_program; intros. monadInv H. split; auto. *) *)
+(* (*   unfold program_of_program; simpl. destruct x; simpl. *) *)
+(* (*   eapply match_transform_partial_program_contextual. eexact EQ. *) *)
+(* (*   intros. apply transl_fundef_spec; auto. *) *)
+(*   (* Qed. *) *)
+(* Admitted. *)
 
-Section PRESERVATION.
+(* Section PRESERVATION. *)
 
-  Variable prog: ChkCsyntax.program.
-  Variable tprog: Csyntax.program.
-  Hypothesis TRANSL: match_prog prog tprog.
+(*   Variable prog: ChkCsyntax.program. *)
+(*   Variable tprog: Csyntax.program. *)
+(*   Hypothesis TRANSL: match_prog prog tprog. *)
 
-  Let ge := ChkCsem.globalenv prog.
-  Let tge := Csem.globalenv tprog.
+(*   Let ge := ChkCsem.globalenv prog. *)
+(*   Let tge := Csem.globalenv tprog. *)
 
-  Lemma senv_preserved:
-    Senv.equiv ge tge.
-  Proof.
-    Admitted.
-(* (Genv.senv_match (proj1 TRANSL)). *)
-
-
-  (** Anti-stuttering measure *)
-
-(** There are some stuttering steps in the translation:
-- The execution of [Sdo a] where [a] is side-effect free,
-  which is three transitions in the source:
-<<
-    Sdo a, k  --->  a, Kdo k ---> rval v, Kdo k ---> Sskip, k
->>
-  but the translation, which is [Sskip], makes no transitions.
-- The reduction [Ecomma (Eval v) r2 --> r2].
-- The reduction [Eparen (Eval v) --> Eval v] in a [For_effects] context.
-
-The following measure decreases for these stuttering steps. *)
-
-Fixpoint esize (a: ChkCsyntax.expr) : nat :=
-  match a with
-  | ChkCsyntax.Eloc _ _ _ => 1%nat
-  | ChkCsyntax.Evar _ _ => 1%nat
-  | ChkCsyntax.Ederef r1 _ => S(esize r1)
-  | ChkCsyntax.Efield l1 _ _ => S(esize l1)
-  | ChkCsyntax.Eval _ _ => O
-  | ChkCsyntax.Evalof l1 _ => S(esize l1)
-  | ChkCsyntax.Eaddrof l1 _ => S(esize l1)
-  | ChkCsyntax.Eunop _ r1 _ => S(esize r1)
-  | ChkCsyntax.Ebinop _ r1 r2 _ => S(esize r1 + esize r2)%nat
-  | ChkCsyntax.Ecast r1 _ => S(esize r1)
-  | ChkCsyntax.Eseqand r1 _ _ => S(esize r1)
-  | ChkCsyntax.Eseqor r1 _ _ => S(esize r1)
-  | ChkCsyntax.Econdition r1 _ _ _ => S(esize r1)
-  | ChkCsyntax.Esizeof _ _ => 1%nat
-  | ChkCsyntax.Ealignof _ _ => 1%nat
-  | ChkCsyntax.Eassign l1 r2 _ => S(esize l1 + esize r2)%nat
-  | ChkCsyntax.Eassignop _ l1 r2 _ _ => S(esize l1 + esize r2)%nat
-  | ChkCsyntax.Epostincr _ l1 _ => S(esize l1)
-  | ChkCsyntax.Ecomma r1 r2 _ => S(esize r1 + esize r2)%nat
-  | ChkCsyntax.Ecall r1 rl2 _ => S(esize r1 + esizelist rl2)%nat
-  | ChkCsyntax.Ebuiltin ef _ rl _ => S(esizelist rl)%nat
-  | ChkCsyntax.Eparen r1 _ _ => S(esize r1)
-  end
-
-with esizelist (el: ChkCsyntax.exprlist) : nat :=
-  match el with
-  | ChkCsyntax.Enil => O
-  | ChkCsyntax.Econs r1 rl2 => (esize r1 + esizelist rl2)%nat
-  end.
-
-Definition measure (st: ChkCsem.state) : nat :=
-  match st with
-  | ChkCsem.ExprState _ r _ _ _ => (esize r + 1)%nat
-  | ChkCsem.State _ ChkCsyntax.Sskip _ _ _ => 0%nat
-  | ChkCsem.State _ (ChkCsyntax.Sdo r) _ _ _ => (esize r + 2)%nat
-  | ChkCsem.State _ (ChkCsyntax.Sifthenelse r _ _) _ _ _ => (esize r + 2)%nat
-  | _ => 0%nat
-  end.
-
-Inductive match_ctx : (ChkCsyntax.expr -> ChkCsyntax.expr) -> (expr -> expr) -> Prop :=
-| match_ctx_transl: forall C tC,
-    (forall e te,
-      tr_expr e te ->
-      tr_expr (C e) (tC te)) ->
-      match_ctx C tC.
-
-Hint Constructors match_ctx.
-
-Inductive match_cont : ChkCsem.cont -> cont -> Prop :=
-  | match_Kstop:
-      match_cont ChkCsem.Kstop Kstop
-  | match_Kdo: forall k tk,
-      match_cont k tk ->
-      match_cont (ChkCsem.Kdo k) (Kdo tk)
-  | match_Kseq: forall s k ts tk,
-      tr_stmt s ts ->
-      match_cont k tk ->
-      match_cont (ChkCsem.Kseq s k) (Kseq ts tk)
-  | match_Kifthenelse: forall s1 s2 k ts1 ts2 tk,
-      tr_stmt s1 ts1 ->
-      tr_stmt s2 ts2 ->
-      match_cont k tk ->
-      match_cont (ChkCsem.Kifthenelse s1 s2 k)
-                 (Kifthenelse ts1 ts2 tk)
-  | match_Kwhile1: forall e te s ts k tk,
-      tr_expr e te ->
-      tr_stmt s ts ->
-      match_cont k tk ->
-      match_cont (ChkCsem.Kwhile1 e s k)
-                 (Kwhile1 te ts tk)
-  | match_Kwhile2: forall e te s ts k tk,
-      tr_expr e te ->
-      tr_stmt s ts ->
-      match_cont k tk ->
-      match_cont (ChkCsem.Kwhile2 e s k)
-                 (Kwhile2 te ts tk)
-  | match_Kdowhile1: forall e te s ts k tk,
-      tr_expr e te ->
-      tr_stmt s ts ->
-      match_cont k tk ->
-      match_cont (ChkCsem.Kdowhile1 e s k)
-                 (Kdowhile1 te ts tk)
-  | match_Kdowhile2: forall e te s ts k tk,
-      tr_expr e te ->
-      tr_stmt s ts ->
-      match_cont k tk ->
-      match_cont (ChkCsem.Kdowhile2 e s k)
-                 (Kdowhile2 te ts tk)
-  | match_Kfor2: forall e te s1 ts1 s2 ts2 k tk,
-      tr_expr e te ->
-      tr_stmt s1 ts1 ->
-      tr_stmt s2 ts2 ->
-      match_cont k tk ->
-      match_cont (ChkCsem.Kfor2 e s1 s2 k)
-                 (Kfor2 te ts1 ts2 tk)
-  | match_Kfor3: forall e te s1 ts1 s2 ts2 k tk,
-      tr_expr e te ->
-      tr_stmt s1 ts1 ->
-      tr_stmt s2 ts2 ->
-      match_cont k tk ->
-      match_cont (ChkCsem.Kfor3 e s1 s2 k)
-                 (Kfor3 te ts1 ts2 tk)
-  | match_Kfor4: forall e te s1 ts1 s2 ts2 k tk,
-      tr_expr e te ->
-      tr_stmt s1 ts1 ->
-      tr_stmt s2 ts2 ->
-      match_cont k tk ->
-      match_cont (ChkCsem.Kfor4 e s1 s2 k)
-                 (Kfor4 te ts1 ts2 tk)
-  | match_Kswitch1: forall ss tss k tk,
-      tr_lblstmts ss tss ->
-      match_cont k tk ->
-      match_cont (ChkCsem.Kswitch1 ss k)
-                 (Kswitch1 tss tk)
-  | match_Kswitch2: forall k tk,
-      match_cont k tk ->
-      match_cont (ChkCsem.Kswitch2 k)
-                 (Kswitch2 tk)
-  | match_Kreturn: forall k tk,
-      match_cont k tk ->
-      match_cont (ChkCsem.Kreturn k)
-                 (Kreturn tk)
-  | match_Kcall: forall f tf e C tC t k tk,
-      tr_function f tf ->
-      match_ctx C tC ->
-      match_cont k tk ->
-      match_cont (ChkCsem.Kcall f e C t k)
-                 (Kcall tf e tC t tk).
-
-Hint Constructors match_cont.
-
-Inductive match_states: ChkCsem.state -> state -> Prop :=
-| match_regstates: forall f tf s ts k tk e m,
-    tr_function f tf ->
-    tr_stmt s ts ->
-    match_cont k tk ->
-      match_states (ChkCsem.State f s k e m)
-                   (State tf ts tk e m)
-| match_exprstates: forall f tf e te k tk env m,
-    tr_function f tf ->
-    tr_expr e te ->
-    match_cont k tk ->
-      match_states (ChkCsem.ExprState f e k env m)
-                   (ExprState tf te tk env m)
-| match_callstates: forall fd tfd args k tk m,
-    tr_fundef fd tfd ->
-    match_cont k tk ->
-    match_states (ChkCsem.Callstate fd args k m)
-                 (Csem.Callstate tfd args tk m)
-| match_returnstates: forall res k tk m,
-    match_cont k tk ->
-    match_states (ChkCsem.Returnstate res k m)
-                 (Csem.Returnstate res tk m)
-| match_stuckstates:
-    match_states ChkCsem.Stuckstate Csem.Stuckstate.
-
-Hint Constructors match_states.
-
-Hint Constructors sstep.
-Hint Constructors estep.
-Hint Constructors tr_stmt.
-Hint Constructors tr_expr.
-
-Lemma transl_not_skip:
-  forall a a',
-    a <> ChkCsyntax.Sskip ->
-    tr_stmt a a' ->
-    a' <> Csyntax.Sskip.
-Proof.
-  intros.
-  induction H0; try discriminate.
-  destruct H. reflexivity.
-Qed.
-
-Hint Resolve transl_not_skip.
-
-Lemma transl_mem:
-  forall m e m',
-    Mem.free_list m (ChkCsem.blocks_of_env ge e) = Some m' ->
-    Mem.free_list m (Csem.blocks_of_env tge e) = Some m'.
-Proof.
-Admitted.
-
-Hint Resolve transl_mem.
-
-Lemma transl_f_cast:
-  forall v1 ty f tf m v2,
-    tr_function f tf ->
-    sem_cast v1 ty (ChkCsyntax.fn_return f) m = Some v2 ->
-    sem_cast v1 ty (Csyntax.fn_return tf) m = Some v2.
-Proof.
-Admitted.
-
-Hint Resolve transl_f_cast.
-
-Lemma transl_call_cont:
-  forall k tk,
-    match_cont k tk ->
-    match_cont (ChkCsem.call_cont k) (Csem.call_cont tk).
-Proof.
-  induction 1; try simpl; eauto.
-Qed.
-
-Hint Resolve transl_call_cont.
-
-Lemma transl_fn_body:
-  forall f tf,
-    tr_function f tf ->
-    tr_stmt (ChkCsyntax.fn_body f) (Csyntax.fn_body tf).
-Proof.
-  destruct 1. assumption.
-Qed.
-
-Hint Resolve transl_fn_body.
-
-Lemma transl_is_call_cont:
-  forall k tk,
-    match_cont k tk ->
-    ChkCsem.is_call_cont k ->
-    is_call_cont tk.
-Proof.
-  induction 1; eauto.
-Qed.
-
-Hint Resolve transl_is_call_cont.
-
-Lemma transl_lblstmts:
-  forall n ss tss,
-    tr_lblstmts ss tss ->
-    tr_stmt (ChkCsem.seq_of_labeled_statement (ChkCsem.select_switch n ss))
-            (seq_of_labeled_statement (select_switch n tss)).
-Proof.
-Admitted.
-
-Hint Resolve transl_lblstmts.
-
-Lemma transl_find_label:
-  forall lbl f tf k tk s' k',
-    tr_function f tf ->
-    match_cont k tk ->
-    ChkCsem.find_label
-      lbl (ChkCsyntax.fn_body f) (ChkCsem.call_cont k) = Some (s', k') ->
-    exists ts' tk', find_label lbl (fn_body tf) (call_cont tk) = Some (ts', tk') /\
-               tr_stmt s' ts' /\ match_cont k' tk'.
-Proof.
-Admitted.
-
-Hint Resolve transl_find_label.
-
-Lemma estep_simulation:
-  forall S1 t S2, ChkCstrategy.estep ge S1 t S2 ->
-  forall S1' (MS: match_states S1 S1'),
-  exists S2', Cstrategy.step tge S1' t S2' /\ match_states S2 S2'.
-Proof.
-Admitted.
-
-Lemma transl_list_norepet:
-  forall f tf,
-    tr_function f tf ->
-    list_norepet
-      (ChkCsyntax.var_names (ChkCsyntax.fn_params f) ++
-                            ChkCsyntax.var_names (ChkCsyntax.fn_vars f)) ->
-    list_norepet (var_names (fn_params tf) ++ var_names (fn_vars tf)).
-Proof.
-  intros.
-  destruct H.
-  destruct f.
-  simpl in *.
-  rewrite H3.
-  rewrite H4.
-  apply H0.
-Qed.
-
-Hint Resolve transl_list_norepet.
-
-Lemma transl_variables:
-  forall f tf m1 e m2 vargs m3,
-    tr_function f tf ->
-    ChkCsem.alloc_variables ge ChkCsem.empty_env m1
-                            (ChkCsyntax.fn_params f ++ ChkCsyntax.fn_vars f) e m2 ->
-    ChkCsem.bind_parameters ge e m2 (ChkCsyntax.fn_params f) vargs m3 ->
-    exists trm2,
-      alloc_variables tge empty_env m1 (fn_params tf ++ fn_vars tf) e trm2 /\
-      bind_parameters tge e trm2 (fn_params tf) vargs m3.
-Proof.
-Admitted.
-
-Lemma transl_external:
-  forall ef vargs m t vres m',
-    external_call ef ge vargs m t vres m' ->
-    external_call ef tge vargs m t vres m'.
-Proof.
-Admitted.
-
-Hint Resolve transl_external.
-
-Lemma sstep_simulation:
-  forall S1 t S2, ChkCsem.sstep ge S1 t S2 ->
-  forall S1' (MS: match_states S1 S1'),
-  exists S2', Cstrategy.step tge S1' t S2' /\ match_states S2 S2'.
-Proof.
-  induction 1; intros; inv MS.
-  - inv H6. econstructor. split; try right; eauto.
-  - inv H6. inv H7. econstructor. split; try right; eauto.
-  - inv H6. econstructor. split; try right; eauto.
-  - inv H6. inv H7. econstructor. split; try right; eauto.
-  - inv H6. inv H7. econstructor. split; try right; eauto.
-  - inv H6. inv H7. econstructor. split; try right; eauto.
-  - inv H6. econstructor. split; try right; eauto.
-  - inv H7. inv H8. destruct b; econstructor; split; try right; eauto.
-  - inv H6. econstructor. split; try right; eauto.
-  - inv H7. inv H8. econstructor. split; try right; eauto.
-  - inv H7. inv H8. econstructor. split; try right; eauto.
-  - inv H; inv H7; inv H8; econstructor; split; try right; eauto.
-  - inv H6. inv H7. econstructor; split; try right; eauto.
-  - inv H6. econstructor. split; try right; eauto.
-  - inv H; inv H7; inv H8; econstructor; split; try right; eauto.
-  - inv H7. inv H8. econstructor. split; try right; eauto.
-  - inv H7. inv H8. econstructor. split; try right; eauto.
-  - inv H6. inv H7. econstructor. split; try right; eauto.
-  - inv H7. econstructor. split; try right; eauto.
-  - inv H6. inv H3. econstructor. split; try right; eauto.
-  - inv H7. inv H8. econstructor. split; try right; eauto.
-  - inv H7. inv H8. econstructor. split; try right; eauto.
-  - inv H; inv H7; inv H8; econstructor; split; try right; eauto.
-  - inv H6. inv H7. econstructor. split; try right; eauto.
-  - inv H6. inv H7. econstructor. split; try right; eauto.
-  - inv H7. econstructor. split; try right; eauto.
-  - inv H6. econstructor. split; try right; eauto.
-  - inv H8. inv H9. econstructor. split; try right; eauto.
-  - inv H8. econstructor. split; try right; eauto.
-  - inv H6. econstructor. split; try right; eauto.
-  - inv H7. inv H8. econstructor. split; try right; eauto.
-  - inv H; inv H7; inv H8; econstructor; split; try right; eauto.
-  - inv H6. inv H7. econstructor. split; try right; eauto.
-  - inv H6. econstructor. split; try right; eauto.
-  - apply transl_find_label with (tf := tf) (tk := tk) in H.
-    inv H. inv H0. inv H. inv H1. inv H7.
-    econstructor; split; try right; eauto. assumption. assumption.
-  - inv H7. econstructor. split; try right; eauto.
-    pose proof transl_variables.
-    specialize (H2 f tf m e m1 vargs m2 H3 H0 H1).
-    inv H2. inv H4.
-    econstructor. eauto.
-    apply H2.
-    apply H5.
-  - inv H5. econstructor. split; try right; eauto.
-  - inv H3. econstructor. split; try right; eauto.
-    inv H7.
-    econstructor. assumption.
-    apply H. econstructor. assumption.
-Qed.
-
-Lemma simulation:
-  forall S1 t S2, ChkCstrategy.step ge S1 t S2 ->
-             forall S1' (MS: match_states S1 S1'),
-             exists S2', Cstrategy.step tge S1' t S2' /\ match_states S2 S2'.
-Proof.
-  intros S1 t S2 STEP.
-  destruct STEP.
-  apply estep_simulation; auto.
-  apply sstep_simulation; auto.
-Qed.
-
-Lemma transl_initial_states:
-  forall S,
-    ChkCsem.initial_state prog S ->
-    exists S', Csem.initial_state tprog S' /\ match_states S S'.
-Proof.
-Admitted.
-
-Lemma transl_final_states:
-  forall S S' r,
-    match_states S S' -> ChkCsem.final_state S r -> Csem.final_state S' r.
-Proof.
-Admitted.
+(*   Lemma senv_preserved: *)
+(*     Senv.equiv ge tge. *)
+(*   Proof. *)
+(*     Admitted. *)
+(* (* (Genv.senv_match (proj1 TRANSL)). *) *)
 
 
-Theorem transl_program_correct:
-  forward_simulation (ChkCstrategy.semantics prog) (Cstrategy.semantics tprog).
-Proof.
-  eapply forward_simulation_step.
-  eapply senv_preserved.
-  eexact transl_initial_states.
-  eexact transl_final_states.
-  exact simulation.
-Qed.
+(*   (** Anti-stuttering measure *) *)
 
-End PRESERVATION.
+(* (** There are some stuttering steps in the translation: *)
+(* - The execution of [Sdo a] where [a] is side-effect free, *)
+(*   which is three transitions in the source: *)
+(* << *)
+(*     Sdo a, k  --->  a, Kdo k ---> rval v, Kdo k ---> Sskip, k *)
+(* >> *)
+(*   but the translation, which is [Sskip], makes no transitions. *)
+(* - The reduction [Ecomma (Eval v) r2 --> r2]. *)
+(* - The reduction [Eparen (Eval v) --> Eval v] in a [For_effects] context. *)
 
-Instance TransfChkCGenLink : TransfLink match_prog.
-Proof.
-  red; intros. eapply Ctypes.link_match_program; eauto.
-  - intros.
-    Local Transparent Linker_fundef.
-    simpl in *; unfold link_fundef in *. inv H3; inv H4; try discriminate.
-    destruct ef; inv H2. exists (Internal tf); split; auto. constructor; auto.
-    destruct ef; inv H2. exists (Internal tf); split; auto. constructor; auto.
-    destruct (external_function_eq ef ef0 && typelist_eq targs targs0 &&
-                                   type_eq tres tres0 && calling_convention_eq cconv cconv0); inv H2.
-    exists (External ef targs tres cconv); split; auto. constructor.
-Qed.
+(* The following measure decreases for these stuttering steps. *) *)
+
+(* Fixpoint esize (a: ChkCsyntax.expr) : nat := *)
+(*   match a with *)
+(*   | ChkCsyntax.Eloc _ _ _ => 1%nat *)
+(*   | ChkCsyntax.Evar _ _ => 1%nat *)
+(*   | ChkCsyntax.Ederef r1 _ => S(esize r1) *)
+(*   | ChkCsyntax.Efield l1 _ _ => S(esize l1) *)
+(*   | ChkCsyntax.Eval _ _ => O *)
+(*   | ChkCsyntax.Evalof l1 _ => S(esize l1) *)
+(*   | ChkCsyntax.Eaddrof l1 _ => S(esize l1) *)
+(*   | ChkCsyntax.Eunop _ r1 _ => S(esize r1) *)
+(*   | ChkCsyntax.Ebinop _ r1 r2 _ => S(esize r1 + esize r2)%nat *)
+(*   | ChkCsyntax.Ecast r1 _ => S(esize r1) *)
+(*   | ChkCsyntax.Eseqand r1 _ _ => S(esize r1) *)
+(*   | ChkCsyntax.Eseqor r1 _ _ => S(esize r1) *)
+(*   | ChkCsyntax.Econdition r1 _ _ _ => S(esize r1) *)
+(*   | ChkCsyntax.Esizeof _ _ => 1%nat *)
+(*   | ChkCsyntax.Ealignof _ _ => 1%nat *)
+(*   | ChkCsyntax.Eassign l1 r2 _ => S(esize l1 + esize r2)%nat *)
+(*   | ChkCsyntax.Eassignop _ l1 r2 _ _ => S(esize l1 + esize r2)%nat *)
+(*   | ChkCsyntax.Epostincr _ l1 _ => S(esize l1) *)
+(*   | ChkCsyntax.Ecomma r1 r2 _ => S(esize r1 + esize r2)%nat *)
+(*   | ChkCsyntax.Ecall r1 rl2 _ => S(esize r1 + esizelist rl2)%nat *)
+(*   | ChkCsyntax.Ebuiltin ef _ rl _ => S(esizelist rl)%nat *)
+(*   | ChkCsyntax.Eparen r1 _ _ => S(esize r1) *)
+(*   end *)
+
+(* with esizelist (el: ChkCsyntax.exprlist) : nat := *)
+(*   match el with *)
+(*   | ChkCsyntax.Enil => O *)
+(*   | ChkCsyntax.Econs r1 rl2 => (esize r1 + esizelist rl2)%nat *)
+(*   end. *)
+
+(* Definition measure (st: ChkCsem.state) : nat := *)
+(*   match st with *)
+(*   | ChkCsem.ExprState _ r _ _ _ => (esize r + 1)%nat *)
+(*   | ChkCsem.State _ ChkCsyntax.Sskip _ _ _ => 0%nat *)
+(*   | ChkCsem.State _ (ChkCsyntax.Sdo r) _ _ _ => (esize r + 2)%nat *)
+(*   | ChkCsem.State _ (ChkCsyntax.Sifthenelse r _ _) _ _ _ => (esize r + 2)%nat *)
+(*   | _ => 0%nat *)
+(*   end. *)
+
+(* Inductive match_ctx : (ChkCsyntax.expr -> ChkCsyntax.expr) -> (expr -> expr) -> Prop := *)
+(* | match_ctx_transl: forall C tC, *)
+(*     (forall e te, *)
+(*       tr_expr e te -> *)
+(*       tr_expr (C e) (tC te)) -> *)
+(*       match_ctx C tC. *)
+
+(* Hint Constructors match_ctx. *)
+
+(* Inductive match_cont : ChkCsem.cont -> cont -> Prop := *)
+(*   | match_Kstop: *)
+(*       match_cont ChkCsem.Kstop Kstop *)
+(*   | match_Kdo: forall k tk, *)
+(*       match_cont k tk -> *)
+(*       match_cont (ChkCsem.Kdo k) (Kdo tk) *)
+(*   | match_Kseq: forall s k ts tk, *)
+(*       tr_stmt s ts -> *)
+(*       match_cont k tk -> *)
+(*       match_cont (ChkCsem.Kseq s k) (Kseq ts tk) *)
+(*   | match_Kifthenelse: forall s1 s2 k ts1 ts2 tk, *)
+(*       tr_stmt s1 ts1 -> *)
+(*       tr_stmt s2 ts2 -> *)
+(*       match_cont k tk -> *)
+(*       match_cont (ChkCsem.Kifthenelse s1 s2 k) *)
+(*                  (Kifthenelse ts1 ts2 tk) *)
+(*   | match_Kwhile1: forall e te s ts k tk, *)
+(*       tr_expr e te -> *)
+(*       tr_stmt s ts -> *)
+(*       match_cont k tk -> *)
+(*       match_cont (ChkCsem.Kwhile1 e s k) *)
+(*                  (Kwhile1 te ts tk) *)
+(*   | match_Kwhile2: forall e te s ts k tk, *)
+(*       tr_expr e te -> *)
+(*       tr_stmt s ts -> *)
+(*       match_cont k tk -> *)
+(*       match_cont (ChkCsem.Kwhile2 e s k) *)
+(*                  (Kwhile2 te ts tk) *)
+(*   | match_Kdowhile1: forall e te s ts k tk, *)
+(*       tr_expr e te -> *)
+(*       tr_stmt s ts -> *)
+(*       match_cont k tk -> *)
+(*       match_cont (ChkCsem.Kdowhile1 e s k) *)
+(*                  (Kdowhile1 te ts tk) *)
+(*   | match_Kdowhile2: forall e te s ts k tk, *)
+(*       tr_expr e te -> *)
+(*       tr_stmt s ts -> *)
+(*       match_cont k tk -> *)
+(*       match_cont (ChkCsem.Kdowhile2 e s k) *)
+(*                  (Kdowhile2 te ts tk) *)
+(*   | match_Kfor2: forall e te s1 ts1 s2 ts2 k tk, *)
+(*       tr_expr e te -> *)
+(*       tr_stmt s1 ts1 -> *)
+(*       tr_stmt s2 ts2 -> *)
+(*       match_cont k tk -> *)
+(*       match_cont (ChkCsem.Kfor2 e s1 s2 k) *)
+(*                  (Kfor2 te ts1 ts2 tk) *)
+(*   | match_Kfor3: forall e te s1 ts1 s2 ts2 k tk, *)
+(*       tr_expr e te -> *)
+(*       tr_stmt s1 ts1 -> *)
+(*       tr_stmt s2 ts2 -> *)
+(*       match_cont k tk -> *)
+(*       match_cont (ChkCsem.Kfor3 e s1 s2 k) *)
+(*                  (Kfor3 te ts1 ts2 tk) *)
+(*   | match_Kfor4: forall e te s1 ts1 s2 ts2 k tk, *)
+(*       tr_expr e te -> *)
+(*       tr_stmt s1 ts1 -> *)
+(*       tr_stmt s2 ts2 -> *)
+(*       match_cont k tk -> *)
+(*       match_cont (ChkCsem.Kfor4 e s1 s2 k) *)
+(*                  (Kfor4 te ts1 ts2 tk) *)
+(*   | match_Kswitch1: forall ss tss k tk, *)
+(*       tr_lblstmts ss tss -> *)
+(*       match_cont k tk -> *)
+(*       match_cont (ChkCsem.Kswitch1 ss k) *)
+(*                  (Kswitch1 tss tk) *)
+(*   | match_Kswitch2: forall k tk, *)
+(*       match_cont k tk -> *)
+(*       match_cont (ChkCsem.Kswitch2 k) *)
+(*                  (Kswitch2 tk) *)
+(*   | match_Kreturn: forall k tk, *)
+(*       match_cont k tk -> *)
+(*       match_cont (ChkCsem.Kreturn k) *)
+(*                  (Kreturn tk) *)
+(*   | match_Kcall: forall f tf e C tC t k tk, *)
+(*       tr_function f tf -> *)
+(*       match_ctx C tC -> *)
+(*       match_cont k tk -> *)
+(*       match_cont (ChkCsem.Kcall f e C t k) *)
+(*                  (Kcall tf e tC t tk). *)
+
+(* Hint Constructors match_cont. *)
+
+(* Inductive match_states: ChkCsem.state -> state -> Prop := *)
+(* | match_regstates: forall f tf s ts k tk e m, *)
+(*     tr_function f tf -> *)
+(*     tr_stmt s ts -> *)
+(*     match_cont k tk -> *)
+(*       match_states (ChkCsem.State f s k e m) *)
+(*                    (State tf ts tk e m) *)
+(* | match_exprstates: forall f tf e te k tk env m, *)
+(*     tr_function f tf -> *)
+(*     tr_expr e te -> *)
+(*     match_cont k tk -> *)
+(*       match_states (ChkCsem.ExprState f e k env m) *)
+(*                    (ExprState tf te tk env m) *)
+(* | match_callstates: forall fd tfd args k tk m, *)
+(*     tr_fundef fd tfd -> *)
+(*     match_cont k tk -> *)
+(*     match_states (ChkCsem.Callstate fd args k m) *)
+(*                  (Csem.Callstate tfd args tk m) *)
+(* | match_returnstates: forall res k tk m, *)
+(*     match_cont k tk -> *)
+(*     match_states (ChkCsem.Returnstate res k m) *)
+(*                  (Csem.Returnstate res tk m) *)
+(* | match_stuckstates: *)
+(*     match_states ChkCsem.Stuckstate Csem.Stuckstate. *)
+
+(* Hint Constructors match_states. *)
+
+(* Hint Constructors sstep. *)
+(* Hint Constructors estep. *)
+(* Hint Constructors tr_stmt. *)
+(* Hint Constructors tr_expr. *)
+
+(* Lemma transl_not_skip: *)
+(*   forall a a', *)
+(*     a <> ChkCsyntax.Sskip -> *)
+(*     tr_stmt a a' -> *)
+(*     a' <> Csyntax.Sskip. *)
+(* Proof. *)
+(*   intros. *)
+(*   induction H0; try discriminate. *)
+(*   destruct H. reflexivity. *)
+(* Qed. *)
+
+(* Hint Resolve transl_not_skip. *)
+
+(* Lemma transl_mem: *)
+(*   forall m e m', *)
+(*     Mem.free_list m (ChkCsem.blocks_of_env ge e) = Some m' -> *)
+(*     Mem.free_list m (Csem.blocks_of_env tge e) = Some m'. *)
+(* Proof. *)
+(* Admitted. *)
+
+(* Hint Resolve transl_mem. *)
+
+(* Lemma transl_f_cast: *)
+(*   forall v1 ty f tf m v2, *)
+(*     tr_function f tf -> *)
+(*     sem_cast v1 ty (ChkCsyntax.fn_return f) m = Some v2 -> *)
+(*     sem_cast v1 ty (Csyntax.fn_return tf) m = Some v2. *)
+(* Proof. *)
+(* Admitted. *)
+
+(* Hint Resolve transl_f_cast. *)
+
+(* Lemma transl_call_cont: *)
+(*   forall k tk, *)
+(*     match_cont k tk -> *)
+(*     match_cont (ChkCsem.call_cont k) (Csem.call_cont tk). *)
+(* Proof. *)
+(*   induction 1; try simpl; eauto. *)
+(* Qed. *)
+
+(* Hint Resolve transl_call_cont. *)
+
+(* Lemma transl_fn_body: *)
+(*   forall f tf, *)
+(*     tr_function f tf -> *)
+(*     tr_stmt (ChkCsyntax.fn_body f) (Csyntax.fn_body tf). *)
+(* Proof. *)
+(*   destruct 1. assumption. *)
+(* Qed. *)
+
+(* Hint Resolve transl_fn_body. *)
+
+(* Lemma transl_is_call_cont: *)
+(*   forall k tk, *)
+(*     match_cont k tk -> *)
+(*     ChkCsem.is_call_cont k -> *)
+(*     is_call_cont tk. *)
+(* Proof. *)
+(*   induction 1; eauto. *)
+(* Qed. *)
+
+(* Hint Resolve transl_is_call_cont. *)
+
+(* Lemma transl_lblstmts: *)
+(*   forall n ss tss, *)
+(*     tr_lblstmts ss tss -> *)
+(*     tr_stmt (ChkCsem.seq_of_labeled_statement (ChkCsem.select_switch n ss)) *)
+(*             (seq_of_labeled_statement (select_switch n tss)). *)
+(* Proof. *)
+(* Admitted. *)
+
+(* Hint Resolve transl_lblstmts. *)
+
+(* Lemma transl_find_label: *)
+(*   forall lbl f tf k tk s' k', *)
+(*     tr_function f tf -> *)
+(*     match_cont k tk -> *)
+(*     ChkCsem.find_label *)
+(*       lbl (ChkCsyntax.fn_body f) (ChkCsem.call_cont k) = Some (s', k') -> *)
+(*     exists ts' tk', find_label lbl (fn_body tf) (call_cont tk) = Some (ts', tk') /\ *)
+(*                tr_stmt s' ts' /\ match_cont k' tk'. *)
+(* Proof. *)
+(* Admitted. *)
+
+(* Hint Resolve transl_find_label. *)
+
+(* Lemma estep_simulation: *)
+(*   forall S1 t S2, ChkCstrategy.estep ge S1 t S2 -> *)
+(*   forall S1' (MS: match_states S1 S1'), *)
+(*   exists S2', Cstrategy.step tge S1' t S2' /\ match_states S2 S2'. *)
+(* Proof. *)
+(* Admitted. *)
+
+(* Lemma transl_list_norepet: *)
+(*   forall f tf, *)
+(*     tr_function f tf -> *)
+(*     list_norepet *)
+(*       (ChkCsyntax.var_names (ChkCsyntax.fn_params f) ++ *)
+(*                             ChkCsyntax.var_names (ChkCsyntax.fn_vars f)) -> *)
+(*     list_norepet (var_names (fn_params tf) ++ var_names (fn_vars tf)). *)
+(* Proof. *)
+(*   intros. *)
+(*   destruct H. *)
+(*   destruct f. *)
+(*   simpl in *. *)
+(*   rewrite H3. *)
+(*   rewrite H4. *)
+(*   apply H0. *)
+(* Qed. *)
+
+(* Hint Resolve transl_list_norepet. *)
+
+(* Lemma transl_variables: *)
+(*   forall f tf m1 e m2 vargs m3, *)
+(*     tr_function f tf -> *)
+(*     ChkCsem.alloc_variables ge ChkCsem.empty_env m1 *)
+(*                             (ChkCsyntax.fn_params f ++ ChkCsyntax.fn_vars f) e m2 -> *)
+(*     ChkCsem.bind_parameters ge e m2 (ChkCsyntax.fn_params f) vargs m3 -> *)
+(*     exists trm2, *)
+(*       alloc_variables tge empty_env m1 (fn_params tf ++ fn_vars tf) e trm2 /\ *)
+(*       bind_parameters tge e trm2 (fn_params tf) vargs m3. *)
+(* Proof. *)
+(* Admitted. *)
+
+(* Lemma transl_external: *)
+(*   forall ef vargs m t vres m', *)
+(*     external_call ef ge vargs m t vres m' -> *)
+(*     external_call ef tge vargs m t vres m'. *)
+(* Proof. *)
+(* Admitted. *)
+
+(* Hint Resolve transl_external. *)
+
+(* Lemma sstep_simulation: *)
+(*   forall S1 t S2, ChkCsem.sstep ge S1 t S2 -> *)
+(*   forall S1' (MS: match_states S1 S1'), *)
+(*   exists S2', Cstrategy.step tge S1' t S2' /\ match_states S2 S2'. *)
+(* Proof. *)
+(*   induction 1; intros; inv MS. *)
+(*   - inv H6. econstructor. split; try right; eauto. *)
+(*   - inv H6. inv H7. econstructor. split; try right; eauto. *)
+(*   - inv H6. econstructor. split; try right; eauto. *)
+(*   - inv H6. inv H7. econstructor. split; try right; eauto. *)
+(*   - inv H6. inv H7. econstructor. split; try right; eauto. *)
+(*   - inv H6. inv H7. econstructor. split; try right; eauto. *)
+(*   - inv H6. econstructor. split; try right; eauto. *)
+(*   - inv H7. inv H8. destruct b; econstructor; split; try right; eauto. *)
+(*   - inv H6. econstructor. split; try right; eauto. *)
+(*   - inv H7. inv H8. econstructor. split; try right; eauto. *)
+(*   - inv H7. inv H8. econstructor. split; try right; eauto. *)
+(*   - inv H; inv H7; inv H8; econstructor; split; try right; eauto. *)
+(*   - inv H6. inv H7. econstructor; split; try right; eauto. *)
+(*   - inv H6. econstructor. split; try right; eauto. *)
+(*   - inv H; inv H7; inv H8; econstructor; split; try right; eauto. *)
+(*   - inv H7. inv H8. econstructor. split; try right; eauto. *)
+(*   - inv H7. inv H8. econstructor. split; try right; eauto. *)
+(*   - inv H6. inv H7. econstructor. split; try right; eauto. *)
+(*   - inv H7. econstructor. split; try right; eauto. *)
+(*   - inv H6. inv H3. econstructor. split; try right; eauto. *)
+(*   - inv H7. inv H8. econstructor. split; try right; eauto. *)
+(*   - inv H7. inv H8. econstructor. split; try right; eauto. *)
+(*   - inv H; inv H7; inv H8; econstructor; split; try right; eauto. *)
+(*   - inv H6. inv H7. econstructor. split; try right; eauto. *)
+(*   - inv H6. inv H7. econstructor. split; try right; eauto. *)
+(*   - inv H7. econstructor. split; try right; eauto. *)
+(*   - inv H6. econstructor. split; try right; eauto. *)
+(*   - inv H8. inv H9. econstructor. split; try right; eauto. *)
+(*   - inv H8. econstructor. split; try right; eauto. *)
+(*   - inv H6. econstructor. split; try right; eauto. *)
+(*   - inv H7. inv H8. econstructor. split; try right; eauto. *)
+(*   - inv H; inv H7; inv H8; econstructor; split; try right; eauto. *)
+(*   - inv H6. inv H7. econstructor. split; try right; eauto. *)
+(*   - inv H6. econstructor. split; try right; eauto. *)
+(*   - apply transl_find_label with (tf := tf) (tk := tk) in H. *)
+(*     inv H. inv H0. inv H. inv H1. inv H7. *)
+(*     econstructor; split; try right; eauto. assumption. assumption. *)
+(*   - inv H7. econstructor. split; try right; eauto. *)
+(*     pose proof transl_variables. *)
+(*     specialize (H2 f tf m e m1 vargs m2 H3 H0 H1). *)
+(*     inv H2. inv H4. *)
+(*     econstructor. eauto. *)
+(*     apply H2. *)
+(*     apply H5. *)
+(*   - inv H5. econstructor. split; try right; eauto. *)
+(*   - inv H3. econstructor. split; try right; eauto. *)
+(*     inv H7. *)
+(*     econstructor. assumption. *)
+(*     apply H. econstructor. assumption. *)
+(* Qed. *)
+
+(* Lemma simulation: *)
+(*   forall S1 t S2, ChkCstrategy.step ge S1 t S2 -> *)
+(*              forall S1' (MS: match_states S1 S1'), *)
+(*              exists S2', Cstrategy.step tge S1' t S2' /\ match_states S2 S2'. *)
+(* Proof. *)
+(*   intros S1 t S2 STEP. *)
+(*   destruct STEP. *)
+(*   apply estep_simulation; auto. *)
+(*   apply sstep_simulation; auto. *)
+(* Qed. *)
+
+(* Lemma transl_initial_states: *)
+(*   forall S, *)
+(*     ChkCsem.initial_state prog S -> *)
+(*     exists S', Csem.initial_state tprog S' /\ match_states S S'. *)
+(* Proof. *)
+(* Admitted. *)
+
+(* Lemma transl_final_states: *)
+(*   forall S S' r, *)
+(*     match_states S S' -> ChkCsem.final_state S r -> Csem.final_state S' r. *)
+(* Proof. *)
+(* Admitted. *)
+
+
+(* Theorem transl_program_correct: *)
+(*   forward_simulation (ChkCstrategy.semantics prog) (Cstrategy.semantics tprog). *)
+(* Proof. *)
+(*   eapply forward_simulation_step. *)
+(*   eapply senv_preserved. *)
+(*   eexact transl_initial_states. *)
+(*   eexact transl_final_states. *)
+(*   exact simulation. *)
+(* Qed. *)
+
+(* End PRESERVATION. *)
+
+(* Instance TransfChkCGenLink : TransfLink match_prog. *)
+(* Proof. *)
+(*   red; intros. eapply Ctypes.link_match_program; eauto. *)
+(*   - intros. *)
+(*     Local Transparent Linker_fundef. *)
+(*     simpl in *; unfold link_fundef in *. inv H3; inv H4; try discriminate. *)
+(*     destruct ef; inv H2. exists (Internal tf); split; auto. constructor; auto. *)
+(*     destruct ef; inv H2. exists (Internal tf); split; auto. constructor; auto. *)
+(*     destruct (external_function_eq ef ef0 && typelist_eq targs targs0 && *)
+(*                                    type_eq tres tres0 && calling_convention_eq cconv cconv0); inv H2. *)
+(*     exists (External ef targs tres cconv); split; auto. constructor. *)
+(* Qed. *)
