cfrontend/ChkCgenspec.v
@@ -14,7 +14,7 @@
 
 Require Import Coqlib Maps Errors Integers Floats.
 Require Import AST Linking Memory.
-Require Import Ctypes Cop ChkCsyntax Csyntax ChkCgen.
+Require Import ChkCtypes Ctypes ChkCop Cop ChkCsyntax Csyntax ChkCgen.
 
 Section SPEC.
 
@@ -33,301 +33,301 @@ Local Open Scope gensym_monad_scope.
   matching the given temporary environment [le].
 *)
 
-Inductive tr_expr: ChkCsyntax.expr -> expr -> Prop :=
-| tr_val: forall v ty,
-    tr_expr (ChkCsyntax.Eval v ty) (Eval v ty)
-| tr_var: forall x ty,
-    tr_expr (ChkCsyntax.Evar x ty) (Evar x ty)
-| tr_field: forall l tl f ty,
-    tr_expr l tl ->
-    tr_expr (ChkCsyntax.Efield l f ty) (Efield tl f ty)
-| tr_valof: forall l tl ty,
-    tr_expr l tl ->
-    tr_expr (ChkCsyntax.Evalof l ty) (Evalof tl ty)
-| tr_deref: forall r tr ty,
-    tr_expr r tr ->
-    tr_expr (ChkCsyntax.Ederef r ty) (Ederef tr ty)
-| tr_addrof: forall l tl ty,
-    tr_expr l tl ->
-    tr_expr (ChkCsyntax.Eaddrof l ty) (Eaddrof tl ty)
-| tr_unop: forall op r tr ty,
-    tr_expr r tr ->
-    tr_expr (ChkCsyntax.Eunop op r ty) (Eunop op tr ty)
-| tr_binop: forall op r1 tr1 r2 tr2 ty,
-    tr_expr r1 tr1 ->
-    tr_expr r2 tr2 ->
-    tr_expr (ChkCsyntax.Ebinop op r1 r2 ty) (Ebinop op tr1 tr2 ty)
-| tr_cast: forall r tr ty,
-    tr_expr r tr ->
-    tr_expr (ChkCsyntax.Ecast r ty) (Ecast tr ty)
-| tr_seqand: forall r1 tr1 r2 tr2 ty,
-    tr_expr r1 tr1 ->
-    tr_expr r2 tr2 ->
-    tr_expr (ChkCsyntax.Eseqand r1 r2 ty) (Eseqand tr1 tr2 ty)
-| tr_seqor: forall r1 tr1 r2 tr2 ty,
-    tr_expr r1 tr1 ->
-    tr_expr r2 tr2 ->
-    tr_expr (ChkCsyntax.Eseqor r1 r2 ty) (Eseqor tr1 tr2 ty)
-| tr_cond: forall r1 tr1 r2 tr2 r3 tr3 ty,
-    tr_expr r1 tr1 ->
-    tr_expr r2 tr2 ->
-    tr_expr r3 tr3 ->
-    tr_expr (ChkCsyntax.Econdition r1 r2 r3 ty) (Econdition tr1 tr2 tr3 ty)
-| tr_sizeof: forall ty' ty,
-    tr_expr (ChkCsyntax.Esizeof ty' ty) (Esizeof ty' ty)
-| tr_alignof: forall ty' ty,
-    tr_expr (ChkCsyntax.Ealignof ty' ty) (Ealignof ty' ty)
-| tr_assign: forall l tl r tr ty,
-    tr_expr l tl ->
-    tr_expr r tr ->
-    tr_expr (ChkCsyntax.Eassign l r ty) (Eassign tl tr ty)
-| tr_assignop: forall op l tl r tr tyres ty,
-    tr_expr l tl ->
-    tr_expr r tr ->
-    tr_expr (ChkCsyntax.Eassignop op l r tyres ty) (Eassignop op tl tr tyres ty)
-| tr_postincr: forall id l tl ty,
-    tr_expr l tl ->
-    tr_expr (ChkCsyntax.Epostincr id l ty) (Epostincr id tl ty)
-| tr_comma: forall r1 tr1 r2 tr2 ty,
-    tr_expr r1 tr1 ->
-    tr_expr r2 tr2 ->
-    tr_expr (ChkCsyntax.Ecomma r1 r2 ty) (Ecomma tr1 tr2 ty)
-| tr_call: forall r1 tr1 rargs trargs ty,
-    tr_expr r1 tr1 ->
-    tr_exprlist rargs trargs ->
-    tr_expr (ChkCsyntax.Ecall r1 rargs ty) (Ecall tr1 trargs ty)
-| tr_builtin: forall ef tyargs rargs trargs ty,
-    tr_exprlist rargs trargs ->
-    tr_expr (ChkCsyntax.Ebuiltin ef tyargs rargs ty) (Ebuiltin ef tyargs trargs ty)
-| tr_loc: forall b ofs ty,
-    tr_expr (ChkCsyntax.Eloc b ofs ty) (Eloc b ofs ty)
-| tr_paren: forall r tr tycast ty,
-    tr_expr r tr ->
-    tr_expr (ChkCsyntax.Eparen r tycast ty) (Eparen tr tycast ty)
+(* Inductive tr_expr: ChkCsyntax.expr -> expr -> Prop := *)
+(* | tr_val: forall v ty, *)
+(*     tr_expr (ChkCsyntax.Eval v ty) (Eval v ty) *)
+(* | tr_var: forall x ty, *)
+(*     tr_expr (ChkCsyntax.Evar x ty) (Evar x ty) *)
+(* | tr_field: forall l tl f ty, *)
+(*     tr_expr l tl -> *)
+(*     tr_expr (ChkCsyntax.Efield l f ty) (Efield tl f ty) *)
+(* | tr_valof: forall l tl ty, *)
+(*     tr_expr l tl -> *)
+(*     tr_expr (ChkCsyntax.Evalof l ty) (Evalof tl ty) *)
+(* | tr_deref: forall r tr ty, *)
+(*     tr_expr r tr -> *)
+(*     tr_expr (ChkCsyntax.Ederef r ty) (Ederef tr ty) *)
+(* | tr_addrof: forall l tl ty, *)
+(*     tr_expr l tl -> *)
+(*     tr_expr (ChkCsyntax.Eaddrof l ty) (Eaddrof tl ty) *)
+(* | tr_unop: forall op r tr ty, *)
+(*     tr_expr r tr -> *)
+(*     tr_expr (ChkCsyntax.Eunop op r ty) (Eunop op tr ty) *)
+(* | tr_binop: forall op r1 tr1 r2 tr2 ty, *)
+(*     tr_expr r1 tr1 -> *)
+(*     tr_expr r2 tr2 -> *)
+(*     tr_expr (ChkCsyntax.Ebinop op r1 r2 ty) (Ebinop op tr1 tr2 ty) *)
+(* | tr_cast: forall r tr ty, *)
+(*     tr_expr r tr -> *)
+(*     tr_expr (ChkCsyntax.Ecast r ty) (Ecast tr ty) *)
+(* | tr_seqand: forall r1 tr1 r2 tr2 ty, *)
+(*     tr_expr r1 tr1 -> *)
+(*     tr_expr r2 tr2 -> *)
+(*     tr_expr (ChkCsyntax.Eseqand r1 r2 ty) (Eseqand tr1 tr2 ty) *)
+(* | tr_seqor: forall r1 tr1 r2 tr2 ty, *)
+(*     tr_expr r1 tr1 -> *)
+(*     tr_expr r2 tr2 -> *)
+(*     tr_expr (ChkCsyntax.Eseqor r1 r2 ty) (Eseqor tr1 tr2 ty) *)
+(* | tr_cond: forall r1 tr1 r2 tr2 r3 tr3 ty, *)
+(*     tr_expr r1 tr1 -> *)
+(*     tr_expr r2 tr2 -> *)
+(*     tr_expr r3 tr3 -> *)
+(*     tr_expr (ChkCsyntax.Econdition r1 r2 r3 ty) (Econdition tr1 tr2 tr3 ty) *)
+(* | tr_sizeof: forall ty' ty, *)
+(*     tr_expr (ChkCsyntax.Esizeof ty' ty) (Esizeof ty' ty) *)
+(* | tr_alignof: forall ty' ty, *)
+(*     tr_expr (ChkCsyntax.Ealignof ty' ty) (Ealignof ty' ty) *)
+(* | tr_assign: forall l tl r tr ty, *)
+(*     tr_expr l tl -> *)
+(*     tr_expr r tr -> *)
+(*     tr_expr (ChkCsyntax.Eassign l r ty) (Eassign tl tr ty) *)
+(* | tr_assignop: forall op l tl r tr tyres ty, *)
+(*     tr_expr l tl -> *)
+(*     tr_expr r tr -> *)
+(*     tr_expr (ChkCsyntax.Eassignop op l r tyres ty) (Eassignop op tl tr tyres ty) *)
+(* | tr_postincr: forall id l tl ty, *)
+(*     tr_expr l tl -> *)
+(*     tr_expr (ChkCsyntax.Epostincr id l ty) (Epostincr id tl ty) *)
+(* | tr_comma: forall r1 tr1 r2 tr2 ty, *)
+(*     tr_expr r1 tr1 -> *)
+(*     tr_expr r2 tr2 -> *)
+(*     tr_expr (ChkCsyntax.Ecomma r1 r2 ty) (Ecomma tr1 tr2 ty) *)
+(* | tr_call: forall r1 tr1 rargs trargs ty, *)
+(*     tr_expr r1 tr1 -> *)
+(*     tr_exprlist rargs trargs -> *)
+(*     tr_expr (ChkCsyntax.Ecall r1 rargs ty) (Ecall tr1 trargs ty) *)
+(* | tr_builtin: forall ef tyargs rargs trargs ty, *)
+(*     tr_exprlist rargs trargs -> *)
+(*     tr_expr (ChkCsyntax.Ebuiltin ef tyargs rargs ty) (Ebuiltin ef tyargs trargs ty) *)
+(* | tr_loc: forall b ofs ty, *)
+(*     tr_expr (ChkCsyntax.Eloc b ofs ty) (Eloc b ofs ty) *)
+(* | tr_paren: forall r tr tycast ty, *)
+(*     tr_expr r tr -> *)
+(*     tr_expr (ChkCsyntax.Eparen r tycast ty) (Eparen tr tycast ty) *)
 
-with tr_exprlist: ChkCsyntax.exprlist -> exprlist -> Prop :=
-| tr_nil:
-    tr_exprlist ChkCsyntax.Enil Enil
-| tr_cons: forall r1 tr1 rl trl,
-    tr_expr r1 tr1 ->
-    tr_exprlist rl trl ->
-    tr_exprlist (ChkCsyntax.Econs r1 rl) (Econs tr1 trl).
+(* with tr_exprlist: ChkCsyntax.exprlist -> exprlist -> Prop := *)
+(* | tr_nil: *)
+(*     tr_exprlist ChkCsyntax.Enil Enil *)
+(* | tr_cons: forall r1 tr1 rl trl, *)
+(*     tr_expr r1 tr1 -> *)
+(*     tr_exprlist rl trl -> *)
+(*     tr_exprlist (ChkCsyntax.Econs r1 rl) (Econs tr1 trl). *)
 
-Hint Constructors tr_expr.
-Hint Constructors tr_exprlist.
+(* Hint Constructors tr_expr. *)
+(* Hint Constructors tr_exprlist. *)
 
-Scheme expr_ind2 := Induction for ChkCsyntax.expr Sort Prop
-  with exprlist_ind2 := Induction for ChkCsyntax.exprlist Sort Prop.
-Combined Scheme expr_exprlist_ind from expr_ind2, exprlist_ind2.
+(* Scheme expr_ind2 := Induction for ChkCsyntax.expr Sort Prop *)
+(*   with exprlist_ind2 := Induction for ChkCsyntax.exprlist Sort Prop. *)
+(* Combined Scheme expr_exprlist_ind from expr_ind2, exprlist_ind2. *)
 
-Inductive tr_stmt: ChkCsyntax.statement -> statement -> Prop :=
-  | tr_skip:
-      tr_stmt ChkCsyntax.Sskip Sskip
-  | tr_do: forall e te,
-      tr_expr e te ->
-      tr_stmt (ChkCsyntax.Sdo e) (Sdo te)
-  | tr_seq: forall s1 s2 ts1 ts2,
-      tr_stmt s1 ts1 ->
-      tr_stmt s2 ts2 ->
-      tr_stmt (ChkCsyntax.Ssequence s1 s2) (Ssequence ts1 ts2)
-  | tr_ifthenelse: forall e te s1 ts1 s2 ts2,
-      tr_expr e te ->
-      tr_stmt s1 ts1 ->
-      tr_stmt s2 ts2 ->
-      tr_stmt (ChkCsyntax.Sifthenelse e s1 s2) (Sifthenelse te ts1 ts2)
-  | tr_while: forall e te s1 ts1,
-      tr_expr e te ->
-      tr_stmt s1 ts1 ->
-      tr_stmt (ChkCsyntax.Swhile e s1) (Swhile te ts1)
-  | tr_dowhile: forall e te s1 ts1,
-      tr_expr e te ->
-      tr_stmt s1 ts1 ->
-      tr_stmt (ChkCsyntax.Sdowhile e s1) (Sdowhile te ts1)
-  | tr_for: forall s1 ts1 e2 te2 s3 ts3 s4 ts4,
-      tr_stmt s1 ts1 ->
-      tr_expr e2 te2 ->
-      tr_stmt s3 ts3 ->
-      tr_stmt s4 ts4 ->
-      tr_stmt (ChkCsyntax.Sfor s1 e2 s3 s4) (Sfor ts1 te2 ts3 ts4)
-  | tr_break:
-      tr_stmt ChkCsyntax.Sbreak Sbreak
-  | tr_continue:
-      tr_stmt ChkCsyntax.Scontinue Scontinue
-  | tr_return_none:
-      tr_stmt (ChkCsyntax.Sreturn None) (Sreturn None)
-  | tr_return_some: forall e te,
-      tr_expr e te ->
-      tr_stmt (ChkCsyntax.Sreturn (Some e)) (Sreturn (Some te))
-  | tr_switch: forall e te ls tls,
-      tr_expr e te ->
-      tr_lblstmts ls tls ->
-      tr_stmt (ChkCsyntax.Sswitch e ls) (Sswitch te tls)
-  | tr_label: forall lbl s ts,
-      tr_stmt s ts ->
-      tr_stmt (ChkCsyntax.Slabel lbl s) (Slabel lbl ts)
-  | tr_goto: forall lbl,
-      tr_stmt (ChkCsyntax.Sgoto lbl) (Sgoto lbl)
+(* Inductive tr_stmt: ChkCsyntax.statement -> statement -> Prop := *)
+(*   | tr_skip: *)
+(*       tr_stmt ChkCsyntax.Sskip Sskip *)
+(*   | tr_do: forall e te, *)
+(*       tr_expr e te -> *)
+(*       tr_stmt (ChkCsyntax.Sdo e) (Sdo te) *)
+(*   | tr_seq: forall s1 s2 ts1 ts2, *)
+(*       tr_stmt s1 ts1 -> *)
+(*       tr_stmt s2 ts2 -> *)
+(*       tr_stmt (ChkCsyntax.Ssequence s1 s2) (Ssequence ts1 ts2) *)
+(*   | tr_ifthenelse: forall e te s1 ts1 s2 ts2, *)
+(*       tr_expr e te -> *)
+(*       tr_stmt s1 ts1 -> *)
+(*       tr_stmt s2 ts2 -> *)
+(*       tr_stmt (ChkCsyntax.Sifthenelse e s1 s2) (Sifthenelse te ts1 ts2) *)
+(*   | tr_while: forall e te s1 ts1, *)
+(*       tr_expr e te -> *)
+(*       tr_stmt s1 ts1 -> *)
+(*       tr_stmt (ChkCsyntax.Swhile e s1) (Swhile te ts1) *)
+(*   | tr_dowhile: forall e te s1 ts1, *)
+(*       tr_expr e te -> *)
+(*       tr_stmt s1 ts1 -> *)
+(*       tr_stmt (ChkCsyntax.Sdowhile e s1) (Sdowhile te ts1) *)
+(*   | tr_for: forall s1 ts1 e2 te2 s3 ts3 s4 ts4, *)
+(*       tr_stmt s1 ts1 -> *)
+(*       tr_expr e2 te2 -> *)
+(*       tr_stmt s3 ts3 -> *)
+(*       tr_stmt s4 ts4 -> *)
+(*       tr_stmt (ChkCsyntax.Sfor s1 e2 s3 s4) (Sfor ts1 te2 ts3 ts4) *)
+(*   | tr_break: *)
+(*       tr_stmt ChkCsyntax.Sbreak Sbreak *)
+(*   | tr_continue: *)
+(*       tr_stmt ChkCsyntax.Scontinue Scontinue *)
+(*   | tr_return_none: *)
+(*       tr_stmt (ChkCsyntax.Sreturn None) (Sreturn None) *)
+(*   | tr_return_some: forall e te, *)
+(*       tr_expr e te -> *)
+(*       tr_stmt (ChkCsyntax.Sreturn (Some e)) (Sreturn (Some te)) *)
+(*   | tr_switch: forall e te ls tls, *)
+(*       tr_expr e te -> *)
+(*       tr_lblstmts ls tls -> *)
+(*       tr_stmt (ChkCsyntax.Sswitch e ls) (Sswitch te tls) *)
+(*   | tr_label: forall lbl s ts, *)
+(*       tr_stmt s ts -> *)
+(*       tr_stmt (ChkCsyntax.Slabel lbl s) (Slabel lbl ts) *)
+(*   | tr_goto: forall lbl, *)
+(*       tr_stmt (ChkCsyntax.Sgoto lbl) (Sgoto lbl) *)
 
-with tr_lblstmts: ChkCsyntax.labeled_statements -> labeled_statements -> Prop :=
-  | tr_ls_nil:
-      tr_lblstmts ChkCsyntax.LSnil LSnil
-  | tr_ls_cons: forall c s ls ts tls,
-      tr_stmt s ts ->
-      tr_lblstmts ls tls ->
-      tr_lblstmts (ChkCsyntax.LScons c s ls) (LScons c ts tls).
+(* with tr_lblstmts: ChkCsyntax.labeled_statements -> labeled_statements -> Prop := *)
+(*   | tr_ls_nil: *)
+(*       tr_lblstmts ChkCsyntax.LSnil LSnil *)
+(*   | tr_ls_cons: forall c s ls ts tls, *)
+(*       tr_stmt s ts -> *)
+(*       tr_lblstmts ls tls -> *)
+(*       tr_lblstmts (ChkCsyntax.LScons c s ls) (LScons c ts tls). *)
 
-Hint Constructors tr_stmt.
-Hint Constructors tr_lblstmts.
+(* Hint Constructors tr_stmt. *)
+(* Hint Constructors tr_lblstmts. *)
 
-(** * Correctness proof with respect to the specification. *)
+(* (** * Correctness proof with respect to the specification. *) *)
 
-(** ** Properties of the monad *)
+(* (** ** Properties of the monad *) *)
 
-Remark bind_inversion:
-  forall (A B: Type) (f: mon A) (g: A -> mon B) (y: B) (z1 z3: generator) I,
-  bind f g z1 = Res y z3 I ->
-  exists x, exists z2, exists I1, exists I2,
-  f z1 = Res x z2 I1 /\ g x z2 = Res y z3 I2.
-Proof.
-  intros until I. unfold bind. destruct (f z1).
-  congruence.
-  caseEq (g a g'); intros; inv H0.
-  econstructor; econstructor; econstructor; econstructor; eauto.
-Qed.
+(* Remark bind_inversion: *)
+(*   forall (A B: Type) (f: mon A) (g: A -> mon B) (y: B) (z1 z3: generator) I, *)
+(*   bind f g z1 = Res y z3 I -> *)
+(*   exists x, exists z2, exists I1, exists I2, *)
+(*   f z1 = Res x z2 I1 /\ g x z2 = Res y z3 I2. *)
+(* Proof. *)
+(*   intros until I. unfold bind. destruct (f z1). *)
+(*   congruence. *)
+(*   caseEq (g a g'); intros; inv H0. *)
+(*   econstructor; econstructor; econstructor; econstructor; eauto. *)
+(* Qed. *)
 
-Remark bind2_inversion:
-  forall (A B Csyntax: Type) (f: mon (A*B)) (g: A -> B -> mon Csyntax) (y: Csyntax) (z1 z3: generator) I,
-  bind2 f g z1 = Res y z3 I ->
-  exists x1, exists x2, exists z2, exists I1, exists I2,
-  f z1 = Res (x1,x2) z2 I1 /\ g x1 x2 z2 = Res y z3 I2.
-Proof.
-  unfold bind2. intros.
-  exploit bind_inversion; eauto.
-  intros [[x1 x2] [z2 [I1 [I2 [P Q]]]]]. simpl in Q.
-  exists x1; exists x2; exists z2; exists I1; exists I2; auto.
-Qed.
+(* Remark bind2_inversion: *)
+(*   forall (A B Csyntax: Type) (f: mon (A*B)) (g: A -> B -> mon Csyntax) (y: Csyntax) (z1 z3: generator) I, *)
+(*   bind2 f g z1 = Res y z3 I -> *)
+(*   exists x1, exists x2, exists z2, exists I1, exists I2, *)
+(*   f z1 = Res (x1,x2) z2 I1 /\ g x1 x2 z2 = Res y z3 I2. *)
+(* Proof. *)
+(*   unfold bind2. intros. *)
+(*   exploit bind_inversion; eauto. *)
+(*   intros [[x1 x2] [z2 [I1 [I2 [P Q]]]]]. simpl in Q. *)
+(*   exists x1; exists x2; exists z2; exists I1; exists I2; auto. *)
+(* Qed. *)
 
-Ltac monadInv1 H :=
-  match type of H with
-  | (Res _ _ _ = Res _ _ _) =>
-      inversion H; clear H; try subst
-  | (@ret _ _ _ = Res _ _ _) =>
-      inversion H; clear H; try subst
-  | (@error _ _ _ = Res _ _ _) =>
-      inversion H
-  | (bind ?F ?G ?Z = Res ?X ?Z' ?I) =>
-      let x := fresh "x" in (
-      let z := fresh "z" in (
-      let I1 := fresh "I" in (
-      let I2 := fresh "I" in (
-      let EQ1 := fresh "EQ" in (
-      let EQ2 := fresh "EQ" in (
-      destruct (bind_inversion _ _ F G X Z Z' I H) as [x [z [I1 [I2 [EQ1 EQ2]]]]];
-      clear H;
-      try (monadInv1 EQ2)))))))
-   | (bind2 ?F ?G ?Z = Res ?X ?Z' ?I) =>
-      let x := fresh "x" in (
-      let y := fresh "y" in (
-      let z := fresh "z" in (
-      let I1 := fresh "I" in (
-      let I2 := fresh "I" in (
-      let EQ1 := fresh "EQ" in (
-      let EQ2 := fresh "EQ" in (
-      destruct (bind2_inversion _ _ _ F G X Z Z' I H) as [x [y [z [I1 [I2 [EQ1 EQ2]]]]]];
-      clear H;
-      try (monadInv1 EQ2))))))))
- end.
+(* Ltac monadInv1 H := *)
+(*   match type of H with *)
+(*   | (Res _ _ _ = Res _ _ _) => *)
+(*       inversion H; clear H; try subst *)
+(*   | (@ret _ _ _ = Res _ _ _) => *)
+(*       inversion H; clear H; try subst *)
+(*   | (@error _ _ _ = Res _ _ _) => *)
+(*       inversion H *)
+(*   | (bind ?F ?G ?Z = Res ?X ?Z' ?I) => *)
+(*       let x := fresh "x" in ( *)
+(*       let z := fresh "z" in ( *)
+(*       let I1 := fresh "I" in ( *)
+(*       let I2 := fresh "I" in ( *)
+(*       let EQ1 := fresh "EQ" in ( *)
+(*       let EQ2 := fresh "EQ" in ( *)
+(*       destruct (bind_inversion _ _ F G X Z Z' I H) as [x [z [I1 [I2 [EQ1 EQ2]]]]]; *)
+(*       clear H; *)
+(*       try (monadInv1 EQ2))))))) *)
+(*    | (bind2 ?F ?G ?Z = Res ?X ?Z' ?I) => *)
+(*       let x := fresh "x" in ( *)
+(*       let y := fresh "y" in ( *)
+(*       let z := fresh "z" in ( *)
+(*       let I1 := fresh "I" in ( *)
+(*       let I2 := fresh "I" in ( *)
+(*       let EQ1 := fresh "EQ" in ( *)
+(*       let EQ2 := fresh "EQ" in ( *)
+(*       destruct (bind2_inversion _ _ _ F G X Z Z' I H) as [x [y [z [I1 [I2 [EQ1 EQ2]]]]]]; *)
+(*       clear H; *)
+(*       try (monadInv1 EQ2)))))))) *)
+(*  end. *)
 
-Ltac monadInv H :=
-  match type of H with
-  | (@ret _ _ _ = Res _ _ _) => monadInv1 H
-  | (@error _ _ _ = Res _ _ _) => monadInv1 H
-  | (bind ?F ?G ?Z = Res ?X ?Z' ?I) => monadInv1 H
-  | (bind2 ?F ?G ?Z = Res ?X ?Z' ?I) => monadInv1 H
-  | (?F _ _ _ _ _ _ _ _ = Res _ _ _) =>
-      ((progress simpl in H) || unfold F in H); monadInv1 H
-  | (?F _ _ _ _ _ _ _ = Res _ _ _) =>
-      ((progress simpl in H) || unfold F in H); monadInv1 H
-  | (?F _ _ _ _ _ _ = Res _ _ _) =>
-      ((progress simpl in H) || unfold F in H); monadInv1 H
-  | (?F _ _ _ _ _ = Res _ _ _) =>
-      ((progress simpl in H) || unfold F in H); monadInv1 H
-  | (?F _ _ _ _ = Res _ _ _) =>
-      ((progress simpl in H) || unfold F in H); monadInv1 H
-  | (?F _ _ _ = Res _ _ _) =>
-      ((progress simpl in H) || unfold F in H); monadInv1 H
-  | (?F _ _ = Res _ _ _) =>
-      ((progress simpl in H) || unfold F in H); monadInv1 H
-  | (?F _ = Res _ _ _) =>
-      ((progress simpl in H) || unfold F in H); monadInv1 H
-  end.
+(* Ltac monadInv H := *)
+(*   match type of H with *)
+(*   | (@ret _ _ _ = Res _ _ _) => monadInv1 H *)
+(*   | (@error _ _ _ = Res _ _ _) => monadInv1 H *)
+(*   | (bind ?F ?G ?Z = Res ?X ?Z' ?I) => monadInv1 H *)
+(*   | (bind2 ?F ?G ?Z = Res ?X ?Z' ?I) => monadInv1 H *)
+(*   | (?F _ _ _ _ _ _ _ _ = Res _ _ _) => *)
+(*       ((progress simpl in H) || unfold F in H); monadInv1 H *)
+(*   | (?F _ _ _ _ _ _ _ = Res _ _ _) => *)
+(*       ((progress simpl in H) || unfold F in H); monadInv1 H *)
+(*   | (?F _ _ _ _ _ _ = Res _ _ _) => *)
+(*       ((progress simpl in H) || unfold F in H); monadInv1 H *)
+(*   | (?F _ _ _ _ _ = Res _ _ _) => *)
+(*       ((progress simpl in H) || unfold F in H); monadInv1 H *)
+(*   | (?F _ _ _ _ = Res _ _ _) => *)
+(*       ((progress simpl in H) || unfold F in H); monadInv1 H *)
+(*   | (?F _ _ _ = Res _ _ _) => *)
+(*       ((progress simpl in H) || unfold F in H); monadInv1 H *)
+(*   | (?F _ _ = Res _ _ _) => *)
+(*       ((progress simpl in H) || unfold F in H); monadInv1 H *)
+(*   | (?F _ = Res _ _ _) => *)
+(*       ((progress simpl in H) || unfold F in H); monadInv1 H *)
+(*   end. *)
 
-Lemma transl_expr_meets_spec:
-  forall e g te g' I,
-  transl_expr e g = Res te g' I ->
-  tr_expr e te.
-Proof.
-  Check expr_exprlist_ind.
-  apply (expr_exprlist_ind
-           (fun e => forall g te g' I, transl_expr e g = Res te g' I -> tr_expr e te)
-           (fun es => forall g tes g' I, transl_exprlist es g = Res tes g' I -> tr_exprlist es tes)); intros;
-    try monadInv H; eauto;
-    try monadInv H0; eauto;
-    try monadInv H1; eauto;
-    try monadInv H2; eauto.
-Qed.
+(* Lemma transl_expr_meets_spec: *)
+(*   forall e g te g' I, *)
+(*   transl_expr e g = Res te g' I -> *)
+(*   tr_expr e te. *)
+(* Proof. *)
+(*   Check expr_exprlist_ind. *)
+(*   apply (expr_exprlist_ind *)
+(*            (fun e => forall g te g' I, transl_expr e g = Res te g' I -> tr_expr e te) *)
+(*            (fun es => forall g tes g' I, transl_exprlist es g = Res tes g' I -> tr_exprlist es tes)); intros; *)
+(*     try monadInv H; eauto; *)
+(*     try monadInv H0; eauto; *)
+(*     try monadInv H1; eauto; *)
+(*     try monadInv H2; eauto. *)
+(* Qed. *)
 
-Lemma transl_stmt_meets_spec:
-  forall s g ts g' I, transl_stmt s g = Res ts g' I -> tr_stmt s ts
-with transl_lblstmt_meets_spec:
-  forall s g ts g' I, transl_lblstmt s g = Res ts g' I -> tr_lblstmts s ts.
-Proof.
-  generalize transl_expr_meets_spec.
-  intros T.
-  clear transl_stmt_meets_spec.
-  intros s. induction s; intros; try destruct o;
-              try monadInv H; try eauto 20.
-  clear transl_lblstmt_meets_spec.
-  intros s. induction s; intros; try monadInv H; try eauto.
-Qed.
+(* Lemma transl_stmt_meets_spec: *)
+(*   forall s g ts g' I, transl_stmt s g = Res ts g' I -> tr_stmt s ts *)
+(* with transl_lblstmt_meets_spec: *)
+(*   forall s g ts g' I, transl_lblstmt s g = Res ts g' I -> tr_lblstmts s ts. *)
+(* Proof. *)
+(*   generalize transl_expr_meets_spec. *)
+(*   intros T. *)
+(*   clear transl_stmt_meets_spec. *)
+(*   intros s. induction s; intros; try destruct o; *)
+(*               try monadInv H; try eauto 20. *)
+(*   clear transl_lblstmt_meets_spec. *)
+(*   intros s. induction s; intros; try monadInv H; try eauto. *)
+(* Qed. *)
 
-(** Relational presentation for the transformation of functions, fundefs, and variables. *)
+(* (** Relational presentation for the transformation of functions, fundefs, and variables. *) *)
 
-Inductive tr_function: ChkCsyntax.function -> Csyntax.function -> Prop :=
-  | tr_function_intro: forall f tf,
-      tr_stmt f.(ChkCsyntax.fn_body) tf.(fn_body) ->
-      fn_return tf = ChkCsyntax.fn_return f ->
-      fn_callconv tf = ChkCsyntax.fn_callconv f ->
-      fn_params tf = ChkCsyntax.fn_params f ->
-      fn_vars tf = ChkCsyntax.fn_vars f ->
-      tr_function f tf.
+(* Inductive tr_function: ChkCsyntax.function -> Csyntax.function -> Prop := *)
+(*   | tr_function_intro: forall f tf, *)
+(*       tr_stmt f.(ChkCsyntax.fn_body) tf.(fn_body) -> *)
+(*       fn_return tf = ChkCsyntax.fn_return f -> *)
+(*       fn_callconv tf = ChkCsyntax.fn_callconv f -> *)
+(*       fn_params tf = ChkCsyntax.fn_params f -> *)
+(*       fn_vars tf = ChkCsyntax.fn_vars f -> *)
+(*       tr_function f tf. *)
 
-Inductive tr_fundef: ChkCsyntax.fundef -> Csyntax.fundef -> Prop :=
-  | tr_internal: forall f tf,
-      tr_function f tf ->
-      tr_fundef (Internal f) (Internal tf)
-  | tr_external: forall ef targs tres cconv,
-      tr_fundef (External ef targs tres cconv) (External ef targs tres cconv).
+(* Inductive tr_fundef: ChkCsyntax.fundef -> Csyntax.fundef -> Prop := *)
+(*   | tr_internal: forall f tf, *)
+(*       tr_function f tf -> *)
+(*       tr_fundef (Internal f) (Internal tf) *)
+(*   | tr_external: forall ef targs tres cconv, *)
+(*       tr_fundef (External ef targs tres cconv) (External ef targs tres cconv). *)
 
-Lemma transl_function_spec:
-  forall f tf,
-  transl_function f = OK tf ->
-  tr_function f tf.
-Proof.
-  unfold transl_function; intros.
-  destruct (transl_stmt (ChkCsyntax.fn_body f) (initial_generator tt)) eqn:T; inv H.
-  constructor; auto. simpl. eapply transl_stmt_meets_spec; eauto.
-Qed.
+(* Lemma transl_function_spec: *)
+(*   forall f tf, *)
+(*   transl_function f = OK tf -> *)
+(*   tr_function f tf. *)
+(* Proof. *)
+(*   unfold transl_function; intros. *)
+(*   destruct (transl_stmt (ChkCsyntax.fn_body f) (initial_generator tt)) eqn:T; inv H. *)
+(*   constructor; auto. simpl. eapply transl_stmt_meets_spec; eauto. *)
+(* Qed. *)
 
-Lemma transl_fundef_spec:
-  forall fd tfd,
-  transl_fundef fd = OK tfd ->
-  tr_fundef fd tfd.
-Proof.
-  unfold transl_fundef; intros.
-  destruct fd; Errors.monadInv H.
-+ constructor. eapply transl_function_spec; eauto.
-+ constructor.
-Qed.
+(* Lemma transl_fundef_spec: *)
+(*   forall fd tfd, *)
+(*   transl_fundef fd = OK tfd -> *)
+(*   tr_fundef fd tfd. *)
+(* Proof. *)
+(*   unfold transl_fundef; intros. *)
+(*   destruct fd; Errors.monadInv H. *)
+(* + constructor. eapply transl_function_spec; eauto. *)
+(* + constructor. *)
+(* Qed. *)
 
 End SPEC.
