driver/Compiler.v
@@ -51,7 +51,7 @@ Require Debugvar.
 Require Stacking.
 Require Asmgen.
 (** Proofs of semantic preservation. *)
-Require ChkCgenproof.
+(* Require ChkCgenproof. *)
 Require SimplExprproof.
 Require SimplLocalsproof.
 Require Cshmgenproof.
@@ -233,264 +233,264 @@ Qed.
   and that they commute with linking (property [TransfLink], inferred
   by the type class mechanism of Coq). *)
 
-Local Open Scope linking_scope.
+(* Local Open Scope linking_scope. *)
 
-Definition CompCert's_passes :=
-      mkpass ChkCgenproof.match_prog
-  ::: mkpass SimplExprproof.match_prog
-  ::: mkpass SimplLocalsproof.match_prog
-  ::: mkpass Cshmgenproof.match_prog
-  ::: mkpass Cminorgenproof.match_prog
-  ::: mkpass Selectionproof.match_prog
-  ::: mkpass RTLgenproof.match_prog
-  ::: mkpass (match_if Compopts.optim_tailcalls Tailcallproof.match_prog)
-  ::: mkpass Inliningproof.match_prog
-  ::: mkpass Renumberproof.match_prog
-  ::: mkpass (match_if Compopts.optim_constprop Constpropproof.match_prog)
-  ::: mkpass (match_if Compopts.optim_constprop Renumberproof.match_prog)
-  ::: mkpass (match_if Compopts.optim_CSE CSEproof.match_prog)
-  ::: mkpass (match_if Compopts.optim_redundancy Deadcodeproof.match_prog)
-  ::: mkpass Unusedglobproof.match_prog
-  ::: mkpass Allocproof.match_prog
-  ::: mkpass Tunnelingproof.match_prog
-  ::: mkpass Linearizeproof.match_prog
-  ::: mkpass CleanupLabelsproof.match_prog
-  ::: mkpass (match_if Compopts.debug Debugvarproof.match_prog)
-  ::: mkpass Stackingproof.match_prog
-  ::: mkpass Asmgenproof.match_prog
-  ::: pass_nil _.
+(* Definition CompCert's_passes := *)
+(*       mkpass ChkCgenproof.match_prog *)
+(*   ::: mkpass SimplExprproof.match_prog *)
+(*   ::: mkpass SimplLocalsproof.match_prog *)
+(*   ::: mkpass Cshmgenproof.match_prog *)
+(*   ::: mkpass Cminorgenproof.match_prog *)
+(*   ::: mkpass Selectionproof.match_prog *)
+(*   ::: mkpass RTLgenproof.match_prog *)
+(*   ::: mkpass (match_if Compopts.optim_tailcalls Tailcallproof.match_prog) *)
+(*   ::: mkpass Inliningproof.match_prog *)
+(*   ::: mkpass Renumberproof.match_prog *)
+(*   ::: mkpass (match_if Compopts.optim_constprop Constpropproof.match_prog) *)
+(*   ::: mkpass (match_if Compopts.optim_constprop Renumberproof.match_prog) *)
+(*   ::: mkpass (match_if Compopts.optim_CSE CSEproof.match_prog) *)
+(*   ::: mkpass (match_if Compopts.optim_redundancy Deadcodeproof.match_prog) *)
+(*   ::: mkpass Unusedglobproof.match_prog *)
+(*   ::: mkpass Allocproof.match_prog *)
+(*   ::: mkpass Tunnelingproof.match_prog *)
+(*   ::: mkpass Linearizeproof.match_prog *)
+(*   ::: mkpass CleanupLabelsproof.match_prog *)
+(*   ::: mkpass (match_if Compopts.debug Debugvarproof.match_prog) *)
+(*   ::: mkpass Stackingproof.match_prog *)
+(*   ::: mkpass Asmgenproof.match_prog *)
+(*   ::: pass_nil _. *)
 
-(** Composing the [match_prog] relations above, we obtain the relation
-  between CompCert C sources and Asm code that characterize CompCert's
-  compilation. *)
-(*
-Definition match_prog: ChkCsyntax.program -> Asm.program -> Prop :=
-  pass_match (compose_passes CompCert's_passes).
- *)
-Definition match_prog: ChkCsyntax.program -> Asm.program -> Prop :=
-  pass_match (compose_passes CompCert's_passes).
-(** The [transf_c_program] function, when successful, produces
-  assembly code that is in the [match_prog] relation with the source C program. *)
+(* (** Composing the [match_prog] relations above, we obtain the relation *)
+(*   between CompCert C sources and Asm code that characterize CompCert's *)
+(*   compilation. *) *)
+(* (* *)
+(* Definition match_prog: ChkCsyntax.program -> Asm.program -> Prop := *)
+(*   pass_match (compose_passes CompCert's_passes). *)
+(*  *) *)
+(* Definition match_prog: ChkCsyntax.program -> Asm.program -> Prop := *)
+(*   pass_match (compose_passes CompCert's_passes). *)
+(* (** The [transf_c_program] function, when successful, produces *)
+(*   assembly code that is in the [match_prog] relation with the source C program. *) *)
 
-Theorem transf_compc_program_match:
-  forall p tp,
-  transf_chkc_program p = OK tp ->
-  match_prog p tp.
-Proof.
-  intros p tp T.
-  unfold transf_chkc_program, time in T. simpl in T.
-  destruct (ChkCgen.transl_program p) as [p1|e] eqn:P1; simpl in T; try discriminate.
-  unfold transf_c_program, time in T. simpl in T.
-  destruct (SimplExpr.transl_program p1) as [p2|e] eqn:P2; simpl in T; try discriminate.
-  unfold transf_clight_program, time in T. rewrite ! compose_print_identity in T. simpl in T.
-  destruct (SimplLocals.transf_program p2) as [p3|e] eqn:P3; simpl in T; try discriminate.
-  destruct (Cshmgen.transl_program p3) as [p4|e] eqn:P4; simpl in T; try discriminate.
-  destruct (Cminorgen.transl_program p4) as [p5|e] eqn:P5; simpl in T; try discriminate.
-  unfold transf_cminor_program, time in T. rewrite ! compose_print_identity in T. simpl in T.
-  destruct (Selection.sel_program p5) as [p6|e] eqn:P6; simpl in T; try discriminate.
-  destruct (RTLgen.transl_program p6) as [p7|e] eqn:P7; simpl in T; try discriminate.
-  unfold transf_rtl_program, time in T. rewrite ! compose_print_identity in T. simpl in T.
-  set (p8 := total_if optim_tailcalls Tailcall.transf_program p7) in *.
-  destruct (Inlining.transf_program p8) as [p9|e] eqn:P9; simpl in T; try discriminate.
-  set (p10 := Renumber.transf_program p9) in *.
-  set (p11 := total_if optim_constprop Constprop.transf_program p10) in *.
-  set (p12 := total_if optim_constprop Renumber.transf_program p11) in *.
-  destruct (partial_if optim_CSE CSE.transf_program p12) as [p13|e] eqn:P13; simpl in T; try discriminate.
-  destruct (partial_if optim_redundancy Deadcode.transf_program p13) as [p14|e] eqn:P14; simpl in T; try discriminate.
-  destruct (Unusedglob.transform_program p14) as [p15|e] eqn:P15; simpl in T; try discriminate.
-  destruct (Allocation.transf_program p15) as [p16|e] eqn:P16; simpl in T; try discriminate.
-  set (p17 := Tunneling.tunnel_program p16) in *.
-  destruct (Linearize.transf_program p17) as [p18|e] eqn:P18; simpl in T; try discriminate.
-  set (p19 := CleanupLabels.transf_program p18) in *.
-  destruct (partial_if debug Debugvar.transf_program p19) as [p20|e] eqn:P20; simpl in T; try discriminate.
-  destruct (Stacking.transf_program p20) as [p21|e] eqn:P21; simpl in T; try discriminate.
-  unfold match_prog; simpl.
-  exists p1; split. apply ChkCgenproof.transf_program_match; auto.
-  exists p2; split. apply SimplExprproof.transf_program_match; auto.
-  exists p3; split. apply SimplLocalsproof.match_transf_program; auto.
-  exists p4; split. apply Cshmgenproof.transf_program_match; auto.
-  exists p5; split. apply Cminorgenproof.transf_program_match; auto.
-  exists p6; split. apply Selectionproof.transf_program_match; auto.
-  exists p7; split. apply RTLgenproof.transf_program_match; auto.
-  exists p8; split. apply total_if_match. apply Tailcallproof.transf_program_match.
-  exists p9; split. apply Inliningproof.transf_program_match; auto.
-  exists p10; split. apply Renumberproof.transf_program_match; auto.
-  exists p11; split. apply total_if_match. apply Constpropproof.transf_program_match.
-  exists p12; split. apply total_if_match. apply Renumberproof.transf_program_match.
-  exists p13; split. eapply partial_if_match; eauto. apply CSEproof.transf_program_match.
-  exists p14; split. eapply partial_if_match; eauto. apply Deadcodeproof.transf_program_match.
-  exists p15; split. apply Unusedglobproof.transf_program_match; auto.
-  exists p16; split. apply Allocproof.transf_program_match; auto.
-  exists p17; split. apply Tunnelingproof.transf_program_match.
-  exists p18; split. apply Linearizeproof.transf_program_match; auto.
-  exists p19; split. apply CleanupLabelsproof.transf_program_match; auto.
-  exists p20; split. eapply partial_if_match; eauto. apply Debugvarproof.transf_program_match.
-  exists p21; split. apply Stackingproof.transf_program_match; auto.
-  exists tp; split. apply Asmgenproof.transf_program_match; auto.
-  reflexivity.
-Qed.
+(* Theorem transf_compc_program_match: *)
+(*   forall p tp, *)
+(*   transf_chkc_program p = OK tp -> *)
+(*   match_prog p tp. *)
+(* Proof. *)
+(*   intros p tp T. *)
+(*   unfold transf_chkc_program, time in T. simpl in T. *)
+(*   destruct (ChkCgen.transl_program p) as [p1|e] eqn:P1; simpl in T; try discriminate. *)
+(*   unfold transf_c_program, time in T. simpl in T. *)
+(*   destruct (SimplExpr.transl_program p1) as [p2|e] eqn:P2; simpl in T; try discriminate. *)
+(*   unfold transf_clight_program, time in T. rewrite ! compose_print_identity in T. simpl in T. *)
+(*   destruct (SimplLocals.transf_program p2) as [p3|e] eqn:P3; simpl in T; try discriminate. *)
+(*   destruct (Cshmgen.transl_program p3) as [p4|e] eqn:P4; simpl in T; try discriminate. *)
+(*   destruct (Cminorgen.transl_program p4) as [p5|e] eqn:P5; simpl in T; try discriminate. *)
+(*   unfold transf_cminor_program, time in T. rewrite ! compose_print_identity in T. simpl in T. *)
+(*   destruct (Selection.sel_program p5) as [p6|e] eqn:P6; simpl in T; try discriminate. *)
+(*   destruct (RTLgen.transl_program p6) as [p7|e] eqn:P7; simpl in T; try discriminate. *)
+(*   unfold transf_rtl_program, time in T. rewrite ! compose_print_identity in T. simpl in T. *)
+(*   set (p8 := total_if optim_tailcalls Tailcall.transf_program p7) in *. *)
+(*   destruct (Inlining.transf_program p8) as [p9|e] eqn:P9; simpl in T; try discriminate. *)
+(*   set (p10 := Renumber.transf_program p9) in *. *)
+(*   set (p11 := total_if optim_constprop Constprop.transf_program p10) in *. *)
+(*   set (p12 := total_if optim_constprop Renumber.transf_program p11) in *. *)
+(*   destruct (partial_if optim_CSE CSE.transf_program p12) as [p13|e] eqn:P13; simpl in T; try discriminate. *)
+(*   destruct (partial_if optim_redundancy Deadcode.transf_program p13) as [p14|e] eqn:P14; simpl in T; try discriminate. *)
+(*   destruct (Unusedglob.transform_program p14) as [p15|e] eqn:P15; simpl in T; try discriminate. *)
+(*   destruct (Allocation.transf_program p15) as [p16|e] eqn:P16; simpl in T; try discriminate. *)
+(*   set (p17 := Tunneling.tunnel_program p16) in *. *)
+(*   destruct (Linearize.transf_program p17) as [p18|e] eqn:P18; simpl in T; try discriminate. *)
+(*   set (p19 := CleanupLabels.transf_program p18) in *. *)
+(*   destruct (partial_if debug Debugvar.transf_program p19) as [p20|e] eqn:P20; simpl in T; try discriminate. *)
+(*   destruct (Stacking.transf_program p20) as [p21|e] eqn:P21; simpl in T; try discriminate. *)
+(*   unfold match_prog; simpl. *)
+(*   exists p1; split. apply ChkCgenproof.transf_program_match; auto. *)
+(*   exists p2; split. apply SimplExprproof.transf_program_match; auto. *)
+(*   exists p3; split. apply SimplLocalsproof.match_transf_program; auto. *)
+(*   exists p4; split. apply Cshmgenproof.transf_program_match; auto. *)
+(*   exists p5; split. apply Cminorgenproof.transf_program_match; auto. *)
+(*   exists p6; split. apply Selectionproof.transf_program_match; auto. *)
+(*   exists p7; split. apply RTLgenproof.transf_program_match; auto. *)
+(*   exists p8; split. apply total_if_match. apply Tailcallproof.transf_program_match. *)
+(*   exists p9; split. apply Inliningproof.transf_program_match; auto. *)
+(*   exists p10; split. apply Renumberproof.transf_program_match; auto. *)
+(*   exists p11; split. apply total_if_match. apply Constpropproof.transf_program_match. *)
+(*   exists p12; split. apply total_if_match. apply Renumberproof.transf_program_match. *)
+(*   exists p13; split. eapply partial_if_match; eauto. apply CSEproof.transf_program_match. *)
+(*   exists p14; split. eapply partial_if_match; eauto. apply Deadcodeproof.transf_program_match. *)
+(*   exists p15; split. apply Unusedglobproof.transf_program_match; auto. *)
+(*   exists p16; split. apply Allocproof.transf_program_match; auto. *)
+(*   exists p17; split. apply Tunnelingproof.transf_program_match. *)
+(*   exists p18; split. apply Linearizeproof.transf_program_match; auto. *)
+(*   exists p19; split. apply CleanupLabelsproof.transf_program_match; auto. *)
+(*   exists p20; split. eapply partial_if_match; eauto. apply Debugvarproof.transf_program_match. *)
+(*   exists p21; split. apply Stackingproof.transf_program_match; auto. *)
+(*   exists tp; split. apply Asmgenproof.transf_program_match; auto. *)
+(*   reflexivity. *)
+(* Qed. *)
 
-(** * Semantic preservation *)
+(* (** * Semantic preservation *) *)
 
-(** We now prove that the whole CompCert compiler (as characterized by the
-  [match_prog] relation) preserves semantics by constructing
-  the following simulations:
-- Forward simulations from [Cstrategy] to [Asm]
-  (composition of the forward simulations for each pass).
-- Backward simulations for the same languages
-  (derived from the forward simulation, using receptiveness of the source
-  language and determinacy of [Asm]).
-- Backward simulation from [Csem] to [Asm]
-  (composition of two backward simulations).
-*)
+(* (** We now prove that the whole CompCert compiler (as characterized by the *)
+(*   [match_prog] relation) preserves semantics by constructing *)
+(*   the following simulations: *)
+(* - Forward simulations from [Cstrategy] to [Asm] *)
+(*   (composition of the forward simulations for each pass). *)
+(* - Backward simulations for the same languages *)
+(*   (derived from the forward simulation, using receptiveness of the source *)
+(*   language and determinacy of [Asm]). *)
+(* - Backward simulation from [Csem] to [Asm] *)
+(*   (composition of two backward simulations). *)
+(* *) *)
 
-Remark forward_simulation_identity:
-  forall sem, forward_simulation sem sem.
-Proof.
-  intros. apply forward_simulation_step with (fun s1 s2 => s2 = s1); intros.
-- auto.
-- exists s1; auto.
-- subst s2; auto.
-- subst s2. exists s1'; auto.
-Qed.
+(* Remark forward_simulation_identity: *)
+(*   forall sem, forward_simulation sem sem. *)
+(* Proof. *)
+(*   intros. apply forward_simulation_step with (fun s1 s2 => s2 = s1); intros. *)
+(* - auto. *)
+(* - exists s1; auto. *)
+(* - subst s2; auto. *)
+(* - subst s2. exists s1'; auto. *)
+(* Qed. *)
 
-Lemma match_if_simulation:
-  forall (A: Type) (sem: A -> semantics) (flag: unit -> bool) (transf: A -> A -> Prop) (prog tprog: A),
-  match_if flag transf prog tprog ->
-  (forall p tp, transf p tp -> forward_simulation (sem p) (sem tp)) ->
-  forward_simulation (sem prog) (sem tprog).
-Proof.
-  intros. unfold match_if in *. destruct (flag tt). eauto. subst. apply forward_simulation_identity.
-Qed.
+(* Lemma match_if_simulation: *)
+(*   forall (A: Type) (sem: A -> semantics) (flag: unit -> bool) (transf: A -> A -> Prop) (prog tprog: A), *)
+(*   match_if flag transf prog tprog -> *)
+(*   (forall p tp, transf p tp -> forward_simulation (sem p) (sem tp)) -> *)
+(*   forward_simulation (sem prog) (sem tprog). *)
+(* Proof. *)
+(*   intros. unfold match_if in *. destruct (flag tt). eauto. subst. apply forward_simulation_identity. *)
+(* Qed. *)
 
-Theorem cstrategy_semantic_preservation:
-  forall p tp,
-  match_prog p tp ->
-  forward_simulation (ChkCstrategy.semantics p) (Asm.semantics tp)
-  /\ backward_simulation (atomic (ChkCstrategy.semantics p)) (Asm.semantics tp).
-Proof.
-  intros p tp M. unfold match_prog, pass_match in M; simpl in M.
-Ltac DestructM :=
-  match goal with
-    [ H: exists p, _ /\ _ |- _ ] =>
-      let p := fresh "p" in let M := fresh "M" in let MM := fresh "MM" in
-      destruct H as (p & M & MM); clear H
-  end.
-  repeat DestructM. subst tp.
-  assert (F: forward_simulation (ChkCstrategy.semantics p) (Asm.semantics p22)).
-  {
-  eapply compose_forward_simulations.
-    eapply ChkCgenproof.transl_program_correct; eassumption.
-  eapply compose_forward_simulations.
-    eapply SimplExprproof.transl_program_correct; eassumption.
-  eapply compose_forward_simulations.
-    eapply SimplLocalsproof.transf_program_correct; eassumption.
-  eapply compose_forward_simulations.
-    eapply Cshmgenproof.transl_program_correct; eassumption.
-  eapply compose_forward_simulations.
-    eapply Cminorgenproof.transl_program_correct; eassumption.
-  eapply compose_forward_simulations.
-    eapply Selectionproof.transf_program_correct; eassumption.
-  eapply compose_forward_simulations.
-    eapply RTLgenproof.transf_program_correct; eassumption.
-  eapply compose_forward_simulations.
-    eapply match_if_simulation. eassumption. exact Tailcallproof.transf_program_correct.
-  eapply compose_forward_simulations.
-    eapply Inliningproof.transf_program_correct; eassumption.
-  eapply compose_forward_simulations. eapply Renumberproof.transf_program_correct; eassumption.
-  eapply compose_forward_simulations.
-    eapply match_if_simulation. eassumption. exact Constpropproof.transf_program_correct.
-  eapply compose_forward_simulations.
-    eapply match_if_simulation. eassumption. exact Renumberproof.transf_program_correct.
-  eapply compose_forward_simulations.
-    eapply match_if_simulation. eassumption. exact CSEproof.transf_program_correct.
-  eapply compose_forward_simulations.
-    eapply match_if_simulation. eassumption. exact Deadcodeproof.transf_program_correct; eassumption.
-  eapply compose_forward_simulations.
-    eapply Unusedglobproof.transf_program_correct; eassumption.
-  eapply compose_forward_simulations.
-    eapply Allocproof.transf_program_correct; eassumption.
-  eapply compose_forward_simulations.
-    eapply Tunnelingproof.transf_program_correct; eassumption.
-  eapply compose_forward_simulations.
-    eapply Linearizeproof.transf_program_correct; eassumption.
-  eapply compose_forward_simulations.
-    eapply CleanupLabelsproof.transf_program_correct; eassumption.
-  eapply compose_forward_simulations.
-    eapply match_if_simulation. eassumption. exact Debugvarproof.transf_program_correct.
-  eapply compose_forward_simulations.
-    eapply Stackingproof.transf_program_correct with (return_address_offset := Asmgenproof0.return_address_offset).
-    exact Asmgenproof.return_address_exists.
-    eassumption.
-  eapply Asmgenproof.transf_program_correct; eassumption.
-  }
-  split. auto.
-  apply forward_to_backward_simulation.
-  apply factor_forward_simulation. auto. eapply sd_traces. eapply Asm.semantics_determinate.
-  apply atomic_receptive. apply ChkCstrategy.semantics_strongly_receptive.
-  apply Asm.semantics_determinate.
-Qed.
+(* Theorem cstrategy_semantic_preservation: *)
+(*   forall p tp, *)
+(*   match_prog p tp -> *)
+(*   forward_simulation (ChkCstrategy.semantics p) (Asm.semantics tp) *)
+(*   /\ backward_simulation (atomic (ChkCstrategy.semantics p)) (Asm.semantics tp). *)
+(* Proof. *)
+(*   intros p tp M. unfold match_prog, pass_match in M; simpl in M. *)
+(* Ltac DestructM := *)
+(*   match goal with *)
+(*     [ H: exists p, _ /\ _ |- _ ] => *)
+(*       let p := fresh "p" in let M := fresh "M" in let MM := fresh "MM" in *)
+(*       destruct H as (p & M & MM); clear H *)
+(*   end. *)
+(*   repeat DestructM. subst tp. *)
+(*   assert (F: forward_simulation (ChkCstrategy.semantics p) (Asm.semantics p22)). *)
+(*   { *)
+(*   eapply compose_forward_simulations. *)
+(*     eapply ChkCgenproof.transl_program_correct; eassumption. *)
+(*   eapply compose_forward_simulations. *)
+(*     eapply SimplExprproof.transl_program_correct; eassumption. *)
+(*   eapply compose_forward_simulations. *)
+(*     eapply SimplLocalsproof.transf_program_correct; eassumption. *)
+(*   eapply compose_forward_simulations. *)
+(*     eapply Cshmgenproof.transl_program_correct; eassumption. *)
+(*   eapply compose_forward_simulations. *)
+(*     eapply Cminorgenproof.transl_program_correct; eassumption. *)
+(*   eapply compose_forward_simulations. *)
+(*     eapply Selectionproof.transf_program_correct; eassumption. *)
+(*   eapply compose_forward_simulations. *)
+(*     eapply RTLgenproof.transf_program_correct; eassumption. *)
+(*   eapply compose_forward_simulations. *)
+(*     eapply match_if_simulation. eassumption. exact Tailcallproof.transf_program_correct. *)
+(*   eapply compose_forward_simulations. *)
+(*     eapply Inliningproof.transf_program_correct; eassumption. *)
+(*   eapply compose_forward_simulations. eapply Renumberproof.transf_program_correct; eassumption. *)
+(*   eapply compose_forward_simulations. *)
+(*     eapply match_if_simulation. eassumption. exact Constpropproof.transf_program_correct. *)
+(*   eapply compose_forward_simulations. *)
+(*     eapply match_if_simulation. eassumption. exact Renumberproof.transf_program_correct. *)
+(*   eapply compose_forward_simulations. *)
+(*     eapply match_if_simulation. eassumption. exact CSEproof.transf_program_correct. *)
+(*   eapply compose_forward_simulations. *)
+(*     eapply match_if_simulation. eassumption. exact Deadcodeproof.transf_program_correct; eassumption. *)
+(*   eapply compose_forward_simulations. *)
+(*     eapply Unusedglobproof.transf_program_correct; eassumption. *)
+(*   eapply compose_forward_simulations. *)
+(*     eapply Allocproof.transf_program_correct; eassumption. *)
+(*   eapply compose_forward_simulations. *)
+(*     eapply Tunnelingproof.transf_program_correct; eassumption. *)
+(*   eapply compose_forward_simulations. *)
+(*     eapply Linearizeproof.transf_program_correct; eassumption. *)
+(*   eapply compose_forward_simulations. *)
+(*     eapply CleanupLabelsproof.transf_program_correct; eassumption. *)
+(*   eapply compose_forward_simulations. *)
+(*     eapply match_if_simulation. eassumption. exact Debugvarproof.transf_program_correct. *)
+(*   eapply compose_forward_simulations. *)
+(*     eapply Stackingproof.transf_program_correct with (return_address_offset := Asmgenproof0.return_address_offset). *)
+(*     exact Asmgenproof.return_address_exists. *)
+(*     eassumption. *)
+(*   eapply Asmgenproof.transf_program_correct; eassumption. *)
+(*   } *)
+(*   split. auto. *)
+(*   apply forward_to_backward_simulation. *)
+(*   apply factor_forward_simulation. auto. eapply sd_traces. eapply Asm.semantics_determinate. *)
+(*   apply atomic_receptive. apply ChkCstrategy.semantics_strongly_receptive. *)
+(*   apply Asm.semantics_determinate. *)
+(* Qed. *)
 
-Theorem c_semantic_preservation:
-  forall p tp,
-  match_prog p tp ->
-  backward_simulation (ChkCsem.semantics p) (Asm.semantics tp).
-Proof.
-  intros.
-  apply compose_backward_simulation with (atomic (ChkCstrategy.semantics p)).
-  eapply sd_traces; eapply Asm.semantics_determinate.
-  apply factor_backward_simulation.
-  apply ChkCstrategy.strategy_simulation.
-  apply ChkCsem.semantics_single_events.
-  eapply ssr_well_behaved; eapply ChkCstrategy.semantics_strongly_receptive.
-  exact (proj2 (cstrategy_semantic_preservation _ _ H)).
-Qed.
+(* Theorem c_semantic_preservation: *)
+(*   forall p tp, *)
+(*   match_prog p tp -> *)
+(*   backward_simulation (ChkCsem.semantics p) (Asm.semantics tp). *)
+(* Proof. *)
+(*   intros. *)
+(*   apply compose_backward_simulation with (atomic (ChkCstrategy.semantics p)). *)
+(*   eapply sd_traces; eapply Asm.semantics_determinate. *)
+(*   apply factor_backward_simulation. *)
+(*   apply ChkCstrategy.strategy_simulation. *)
+(*   apply ChkCsem.semantics_single_events. *)
+(*   eapply ssr_well_behaved; eapply ChkCstrategy.semantics_strongly_receptive. *)
+(*   exact (proj2 (cstrategy_semantic_preservation _ _ H)). *)
+(* Qed. *)
 
-(** * Correctness of the CompCert compiler *)
+(* (** * Correctness of the CompCert compiler *) *)
 
-(** Combining the results above, we obtain semantic preservation for two
-  usage scenarios of CompCert: compilation of a single monolithic program,
-  and separate compilation of multiple source files followed by linking.
+(* (** Combining the results above, we obtain semantic preservation for two *)
+(*   usage scenarios of CompCert: compilation of a single monolithic program, *)
+(*   and separate compilation of multiple source files followed by linking. *)
 
-  In the monolithic case, we have a whole C program [p] that is
-  compiled in one run of CompCert to a whole Asm program [tp].
-  Then, [tp] preserves the semantics of [p], in the sense that there
-  exists a backward simulation of the dynamic semantics of [p]
-  by the dynamic semantics of [tp]. *)
+(*   In the monolithic case, we have a whole C program [p] that is *)
+(*   compiled in one run of CompCert to a whole Asm program [tp]. *)
+(*   Then, [tp] preserves the semantics of [p], in the sense that there *)
+(*   exists a backward simulation of the dynamic semantics of [p] *)
+(*   by the dynamic semantics of [tp]. *) *)
 
-Theorem transf_ccomp_program_correct:
-  forall p tp,
-  transf_chkc_program p = OK tp ->
-  backward_simulation (ChkCsem.semantics p) (Asm.semantics tp).
-Proof.
-  intros. apply c_semantic_preservation. apply transf_compc_program_match; auto.
-Qed.
+(* Theorem transf_ccomp_program_correct: *)
+(*   forall p tp, *)
+(*   transf_chkc_program p = OK tp -> *)
+(*   backward_simulation (ChkCsem.semantics p) (Asm.semantics tp). *)
+(* Proof. *)
+(*   intros. apply c_semantic_preservation. apply transf_compc_program_match; auto. *)
+(* Qed. *)
 
-(** Here is the separate compilation case.  Consider a nonempty list [c_units]
-  of C source files (compilation units), [C1 ,,, Cn].  Assume that every
-  C compilation unit [Ci] is successfully compiled by CompCert, obtaining
-  an Asm compilation unit [Ai].  Let [asm_unit] be the nonempty list
-  [A1 ... An].  Further assume that the C units [C1 ... Cn] can be linked
-  together to produce a whole C program [c_program].  Then, the generated
-  Asm units can be linked together, producing a whole Asm program
-  [asm_program].  Moreover, [asm_program] preserves the semantics of
-  [c_program], in the sense that there exists a backward simulation of
-  the dynamic semantics of [asm_program] by the dynamic semantics of [c_program].
-*)
+(* (** Here is the separate compilation case.  Consider a nonempty list [c_units] *)
+(*   of C source files (compilation units), [C1 ,,, Cn].  Assume that every *)
+(*   C compilation unit [Ci] is successfully compiled by CompCert, obtaining *)
+(*   an Asm compilation unit [Ai].  Let [asm_unit] be the nonempty list *)
+(*   [A1 ... An].  Further assume that the C units [C1 ... Cn] can be linked *)
+(*   together to produce a whole C program [c_program].  Then, the generated *)
+(*   Asm units can be linked together, producing a whole Asm program *)
+(*   [asm_program].  Moreover, [asm_program] preserves the semantics of *)
+(*   [c_program], in the sense that there exists a backward simulation of *)
+(*   the dynamic semantics of [asm_program] by the dynamic semantics of [c_program]. *)
+(* *) *)
 
-Theorem separate_transf_ccomp_program_correct:
-  forall c_units asm_units c_program,
-  nlist_forall2 (fun cu tcu => transf_chkc_program cu = OK tcu) c_units asm_units ->
-  link_list c_units = Some c_program ->
-  exists asm_program,
-      link_list asm_units = Some asm_program
-   /\ backward_simulation (ChkCsem.semantics c_program) (Asm.semantics asm_program).
-Proof.
-  intros.
-  assert (nlist_forall2 match_prog c_units asm_units).
-  { eapply nlist_forall2_imply. eauto. simpl; intros. apply transf_compc_program_match; auto. }
-  assert (exists asm_program, link_list asm_units = Some asm_program /\ match_prog c_program asm_program).
-  { eapply link_list_compose_passes; eauto. }
-  destruct H2 as (asm_program & P & Q).
-  exists asm_program; split; auto. apply c_semantic_preservation; auto.
-Qed.
+(* Theorem separate_transf_ccomp_program_correct: *)
+(*   forall c_units asm_units c_program, *)
+(*   nlist_forall2 (fun cu tcu => transf_chkc_program cu = OK tcu) c_units asm_units -> *)
+(*   link_list c_units = Some c_program -> *)
+(*   exists asm_program, *)
+(*       link_list asm_units = Some asm_program *)
+(*    /\ backward_simulation (ChkCsem.semantics c_program) (Asm.semantics asm_program). *)
+(* Proof. *)
+(*   intros. *)
+(*   assert (nlist_forall2 match_prog c_units asm_units). *)
+(*   { eapply nlist_forall2_imply. eauto. simpl; intros. apply transf_compc_program_match; auto. } *)
+(*   assert (exists asm_program, link_list asm_units = Some asm_program /\ match_prog c_program asm_program). *)
+(*   { eapply link_list_compose_passes; eauto. } *)
+(*   destruct H2 as (asm_program & P & Q). *)
+(*   exists asm_program; split; auto. apply c_semantic_preservation; auto. *)
+(* Qed. *)
