driver/Complements.v
@@ -18,287 +18,287 @@ Require Import AST Linking Events Smallstep Behaviors.
 Require Import Csyntax Csem Cstrategy Asm ChkCsem ChkCstrategy.
 Require Import Compiler.
 
-(** * Preservation of whole-program behaviors *)
+(* (** * Preservation of whole-program behaviors *) *)
 
-(** From the simulation diagrams proved in file [Compiler]. it follows that
-  whole-program observable behaviors are preserved in the following sense.
-  First, every behavior of the generated assembly code is matched by
-  a behavior of the source C code.  The behavior [beh] of the assembly
-  code is either identical to the behavior [beh'] of the source C code
-  or ``improves upon'' [beh']  by replacing a ``going wrong'' behavior
-  with a more defined behavior. *)
+(* (** From the simulation diagrams proved in file [Compiler]. it follows that *)
+(*   whole-program observable behaviors are preserved in the following sense. *)
+(*   First, every behavior of the generated assembly code is matched by *)
+(*   a behavior of the source C code.  The behavior [beh] of the assembly *)
+(*   code is either identical to the behavior [beh'] of the source C code *)
+(*   or ``improves upon'' [beh']  by replacing a ``going wrong'' behavior *)
+(*   with a more defined behavior. *) *)
 
-Theorem transf_c_program_preservation:
-  forall p tp beh,
-  transf_chkc_program p = OK tp ->
-  program_behaves (Asm.semantics tp) beh ->
-  exists beh', program_behaves (ChkCsem.semantics p) beh' /\ behavior_improves beh' beh.
-Proof.
-  intros. eapply backward_simulation_behavior_improves; eauto.
-  apply transf_ccomp_program_correct; auto.
-Qed.
+(* Theorem transf_c_program_preservation: *)
+(*   forall p tp beh, *)
+(*   transf_chkc_program p = OK tp -> *)
+(*   program_behaves (Asm.semantics tp) beh -> *)
+(*   exists beh', program_behaves (ChkCsem.semantics p) beh' /\ behavior_improves beh' beh. *)
+(* Proof. *)
+(*   intros. eapply backward_simulation_behavior_improves; eauto. *)
+(*   apply transf_ccomp_program_correct; auto. *)
+(* Qed. *)
 
-(** As a corollary, if the source C code cannot go wrong, i.e. is free of
-  undefined behaviors, the behavior of the generated assembly code is
-  one of the possible behaviors of the source C code. *)
+(* (** As a corollary, if the source C code cannot go wrong, i.e. is free of *)
+(*   undefined behaviors, the behavior of the generated assembly code is *)
+(*   one of the possible behaviors of the source C code. *) *)
 
-Theorem transf_c_program_is_refinement:
-  forall p tp,
-  transf_chkc_program p = OK tp ->
-  (forall beh, program_behaves (ChkCsem.semantics p) beh -> not_wrong beh) ->
-  (forall beh, program_behaves (Asm.semantics tp) beh -> program_behaves (ChkCsem.semantics p) beh).
-Proof.
-  intros. eapply backward_simulation_same_safe_behavior; eauto.
-  apply transf_ccomp_program_correct; auto.
-Qed.
+(* Theorem transf_c_program_is_refinement: *)
+(*   forall p tp, *)
+(*   transf_chkc_program p = OK tp -> *)
+(*   (forall beh, program_behaves (ChkCsem.semantics p) beh -> not_wrong beh) -> *)
+(*   (forall beh, program_behaves (Asm.semantics tp) beh -> program_behaves (ChkCsem.semantics p) beh). *)
+(* Proof. *)
+(*   intros. eapply backward_simulation_same_safe_behavior; eauto. *)
+(*   apply transf_ccomp_program_correct; auto. *)
+(* Qed. *)
 
-(** If we consider the C evaluation strategy implemented by the compiler,
-  we get stronger preservation results. *)
+(* (** If we consider the C evaluation strategy implemented by the compiler, *)
+(*   we get stronger preservation results. *) *)
 
-Theorem transf_cstrategy_program_preservation:
-  forall p tp,
-  transf_chkc_program p = OK tp ->
-  (forall beh, program_behaves (ChkCstrategy.semantics p) beh ->
-     exists beh', program_behaves (Asm.semantics tp) beh' /\ behavior_improves beh beh')
-/\(forall beh, program_behaves (Asm.semantics tp) beh ->
-     exists beh', program_behaves (ChkCstrategy.semantics p) beh' /\ behavior_improves beh' beh)
-/\(forall beh, not_wrong beh ->
-     program_behaves (ChkCstrategy.semantics p) beh -> program_behaves (Asm.semantics tp) beh)
-/\(forall beh,
-     (forall beh', program_behaves (ChkCstrategy.semantics p) beh' -> not_wrong beh') ->
-     program_behaves (Asm.semantics tp) beh ->
-     program_behaves (ChkCstrategy.semantics p) beh).
-Proof.
-  assert (WBT: forall p, well_behaved_traces (semantics p)).
-    intros. eapply ssr_well_behaved. apply ChkCstrategy.semantics_strongly_receptive.
-  intros.
-  assert (MATCH: match_prog p tp) by (apply transf_compc_program_match; auto).
-  intuition auto.
-  eapply forward_simulation_behavior_improves; eauto.
-    apply (proj1 (cstrategy_semantic_preservation _ _ MATCH)).
-  exploit backward_simulation_behavior_improves.
-    apply (proj2 (cstrategy_semantic_preservation _ _ MATCH)).
-    eauto.
-  intros [beh1 [A B]]. exists beh1; split; auto. rewrite atomic_behaviors; auto.
-  eapply forward_simulation_same_safe_behavior; eauto.
-    apply (proj1 (cstrategy_semantic_preservation _ _ MATCH)).
-  exploit backward_simulation_same_safe_behavior.
-    apply (proj2 (cstrategy_semantic_preservation _ _ MATCH)).
-    intros. rewrite <- atomic_behaviors in H2; eauto. eauto.
-    intros. rewrite atomic_behaviors; auto.
-Qed.
+(* Theorem transf_cstrategy_program_preservation: *)
+(*   forall p tp, *)
+(*   transf_chkc_program p = OK tp -> *)
+(*   (forall beh, program_behaves (ChkCstrategy.semantics p) beh -> *)
+(*      exists beh', program_behaves (Asm.semantics tp) beh' /\ behavior_improves beh beh') *)
+(* /\(forall beh, program_behaves (Asm.semantics tp) beh -> *)
+(*      exists beh', program_behaves (ChkCstrategy.semantics p) beh' /\ behavior_improves beh' beh) *)
+(* /\(forall beh, not_wrong beh -> *)
+(*      program_behaves (ChkCstrategy.semantics p) beh -> program_behaves (Asm.semantics tp) beh) *)
+(* /\(forall beh, *)
+(*      (forall beh', program_behaves (ChkCstrategy.semantics p) beh' -> not_wrong beh') -> *)
+(*      program_behaves (Asm.semantics tp) beh -> *)
+(*      program_behaves (ChkCstrategy.semantics p) beh). *)
+(* Proof. *)
+(*   assert (WBT: forall p, well_behaved_traces (semantics p)). *)
+(*     intros. eapply ssr_well_behaved. apply ChkCstrategy.semantics_strongly_receptive. *)
+(*   intros. *)
+(*   assert (MATCH: match_prog p tp) by (apply transf_compc_program_match; auto). *)
+(*   intuition auto. *)
+(*   eapply forward_simulation_behavior_improves; eauto. *)
+(*     apply (proj1 (cstrategy_semantic_preservation _ _ MATCH)). *)
+(*   exploit backward_simulation_behavior_improves. *)
+(*     apply (proj2 (cstrategy_semantic_preservation _ _ MATCH)). *)
+(*     eauto. *)
+(*   intros [beh1 [A B]]. exists beh1; split; auto. rewrite atomic_behaviors; auto. *)
+(*   eapply forward_simulation_same_safe_behavior; eauto. *)
+(*     apply (proj1 (cstrategy_semantic_preservation _ _ MATCH)). *)
+(*   exploit backward_simulation_same_safe_behavior. *)
+(*     apply (proj2 (cstrategy_semantic_preservation _ _ MATCH)). *)
+(*     intros. rewrite <- atomic_behaviors in H2; eauto. eauto. *)
+(*     intros. rewrite atomic_behaviors; auto. *)
+(* Qed. *)
 
-(** We can also use the alternate big-step semantics for [Cstrategy]
-  to establish behaviors of the generated assembly code. *)
+(* (** We can also use the alternate big-step semantics for [Cstrategy] *)
+(*   to establish behaviors of the generated assembly code. *) *)
 
-Theorem bigstep_cstrategy_preservation:
-  forall p tp,
-  transf_chkc_program p = OK tp ->
-  (forall t r,
-     ChkCstrategy.bigstep_program_terminates p t r ->
-     program_behaves (Asm.semantics tp) (Terminates t r))
-/\(forall T,
-     ChkCstrategy.bigstep_program_diverges p T ->
-       program_behaves (Asm.semantics tp) (Reacts T)
-    \/ exists t, program_behaves (Asm.semantics tp) (Diverges t) /\ traceinf_prefix t T).
-Proof.
-  intuition.
-  apply transf_cstrategy_program_preservation with p; auto. red; auto.
-  apply behavior_bigstep_terminates with (ChkCstrategy.bigstep_semantics p); auto.
-  apply ChkCstrategy.bigstep_semantics_sound.
-  exploit (behavior_bigstep_diverges (ChkCstrategy.bigstep_semantics_sound p)). eassumption.
-  intros [A | [t [A B]]].
-  left. apply transf_cstrategy_program_preservation with p; auto. red; auto.
-  right; exists t; split; auto. apply transf_cstrategy_program_preservation with p; auto. red; auto.
-Qed.
+(* Theorem bigstep_cstrategy_preservation: *)
+(*   forall p tp, *)
+(*   transf_chkc_program p = OK tp -> *)
+(*   (forall t r, *)
+(*      ChkCstrategy.bigstep_program_terminates p t r -> *)
+(*      program_behaves (Asm.semantics tp) (Terminates t r)) *)
+(* /\(forall T, *)
+(*      ChkCstrategy.bigstep_program_diverges p T -> *)
+(*        program_behaves (Asm.semantics tp) (Reacts T) *)
+(*     \/ exists t, program_behaves (Asm.semantics tp) (Diverges t) /\ traceinf_prefix t T). *)
+(* Proof. *)
+(*   intuition. *)
+(*   apply transf_cstrategy_program_preservation with p; auto. red; auto. *)
+(*   apply behavior_bigstep_terminates with (ChkCstrategy.bigstep_semantics p); auto. *)
+(*   apply ChkCstrategy.bigstep_semantics_sound. *)
+(*   exploit (behavior_bigstep_diverges (ChkCstrategy.bigstep_semantics_sound p)). eassumption. *)
+(*   intros [A | [t [A B]]]. *)
+(*   left. apply transf_cstrategy_program_preservation with p; auto. red; auto. *)
+(*   right; exists t; split; auto. apply transf_cstrategy_program_preservation with p; auto. red; auto. *)
+(* Qed. *)
 
-(** * Satisfaction of specifications *)
+(* (** * Satisfaction of specifications *) *)
 
-(** The second additional results shows that if all executions
-  of the source C program satisfies a given specification,
-  then all executions of the produced Asm program satisfy
-  this specification as well.  *)
+(* (** The second additional results shows that if all executions *)
+(*   of the source C program satisfies a given specification, *)
+(*   then all executions of the produced Asm program satisfy *)
+(*   this specification as well.  *) *)
 
-(** The specifications we consider here are sets of observable
-  behaviors, representing the good behaviors a program is expected
-  to have.  A specification can be as simple as
-  ``the program does not go wrong'' or as precise as
-  ``the program prints a prime number then terminates with code 0''.
-  As usual in Coq, sets of behaviors are represented as predicates
-  [program_behavior -> Prop]. *)
+(* (** The specifications we consider here are sets of observable *)
+(*   behaviors, representing the good behaviors a program is expected *)
+(*   to have.  A specification can be as simple as *)
+(*   ``the program does not go wrong'' or as precise as *)
+(*   ``the program prints a prime number then terminates with code 0''. *)
+(*   As usual in Coq, sets of behaviors are represented as predicates *)
+(*   [program_behavior -> Prop]. *) *)
 
-Definition specification := program_behavior -> Prop.
+(* Definition specification := program_behavior -> Prop. *)
 
-(** A program satisfies a specification if all its observable behaviors
-  are in the specification. *)
+(* (** A program satisfies a specification if all its observable behaviors *)
+(*   are in the specification. *) *)
 
-Definition c_program_satisfies_spec (p: ChkCsyntax.program) (spec: specification): Prop :=
-  forall beh,  program_behaves (ChkCsem.semantics p) beh -> spec beh.
-Definition asm_program_satisfies_spec (p: Asm.program) (spec: specification): Prop :=
-  forall beh,  program_behaves (Asm.semantics p) beh -> spec beh.
+(* Definition c_program_satisfies_spec (p: ChkCsyntax.program) (spec: specification): Prop := *)
+(*   forall beh,  program_behaves (ChkCsem.semantics p) beh -> spec beh. *)
+(* Definition asm_program_satisfies_spec (p: Asm.program) (spec: specification): Prop := *)
+(*   forall beh,  program_behaves (Asm.semantics p) beh -> spec beh. *)
   
-(** It is not always the case that if the source program satisfies a
-  specification, then the generated assembly code satisfies it as
-  well.  For example, if the specification is ``the program goes wrong
-  on an undefined behavior'', a C source that goes wrong satisfies
-  this specification but can be compiled into Asm code that does not
-  go wrong and therefore does not satisfy the specification.
+(* (** It is not always the case that if the source program satisfies a *)
+(*   specification, then the generated assembly code satisfies it as *)
+(*   well.  For example, if the specification is ``the program goes wrong *)
+(*   on an undefined behavior'', a C source that goes wrong satisfies *)
+(*   this specification but can be compiled into Asm code that does not *)
+(*   go wrong and therefore does not satisfy the specification. *)
 
-  For this reason, we restrict ourselves to safety-enforcing specifications:
-  specifications that exclude ``going wrong'' behaviors and are satisfied
-  only by programs that execute safely. *)
+(*   For this reason, we restrict ourselves to safety-enforcing specifications: *)
+(*   specifications that exclude ``going wrong'' behaviors and are satisfied *)
+(*   only by programs that execute safely. *) *)
 
-Definition safety_enforcing_specification (spec: specification): Prop :=
-  forall beh, spec beh -> not_wrong beh.
+(* Definition safety_enforcing_specification (spec: specification): Prop := *)
+(*   forall beh, spec beh -> not_wrong beh. *)
 
-(** As the main result of this section, we show that CompCert
-  compilation preserves safety-enforcing specifications: 
-  any such specification that is satisfied by the source C program is
-  always satisfied by the generated assembly code. *)
+(* (** As the main result of this section, we show that CompCert *)
+(*   compilation preserves safety-enforcing specifications:  *)
+(*   any such specification that is satisfied by the source C program is *)
+(*   always satisfied by the generated assembly code. *) *)
 
-Theorem transf_c_program_preserves_spec:
-  forall p tp spec,
-  transf_chkc_program p = OK tp ->
-  safety_enforcing_specification spec ->
-  c_program_satisfies_spec p spec ->
-  asm_program_satisfies_spec tp spec.
-Proof.
-  intros p tp spec TRANSF SES CSAT; red; intros beh AEXEC.
-  exploit transf_c_program_preservation; eauto. intros (beh' & CEXEC & IMPR).
-  apply CSAT in CEXEC. destruct IMPR as [EQ | [t [A B]]].
-- congruence.
-- subst beh'. apply SES in CEXEC. contradiction. 
-Qed.
+(* Theorem transf_c_program_preserves_spec: *)
+(*   forall p tp spec, *)
+(*   transf_chkc_program p = OK tp -> *)
+(*   safety_enforcing_specification spec -> *)
+(*   c_program_satisfies_spec p spec -> *)
+(*   asm_program_satisfies_spec tp spec. *)
+(* Proof. *)
+(*   intros p tp spec TRANSF SES CSAT; red; intros beh AEXEC. *)
+(*   exploit transf_c_program_preservation; eauto. intros (beh' & CEXEC & IMPR). *)
+(*   apply CSAT in CEXEC. destruct IMPR as [EQ | [t [A B]]]. *)
+(* - congruence. *)
+(* - subst beh'. apply SES in CEXEC. contradiction.  *)
+(* Qed. *)
 
-(** Safety-enforcing specifications are not the only good properties
-  of source programs that are preserved by compilation.  Another example
-  of a property that is preserved is the ``initial trace'' property:
-  all executions of the program start by producing an expected trace
-  of I/O actions, representing the good behavior expected from the program.
-  After that, the program may terminate, or continue running, or go wrong
-  on an undefined behavior.  What matters is that the program produced
-  the expected trace at the beginning of its execution.  This is a typical
-  liveness property, and it is preserved by compilation. *)
+(* (** Safety-enforcing specifications are not the only good properties *)
+(*   of source programs that are preserved by compilation.  Another example *)
+(*   of a property that is preserved is the ``initial trace'' property: *)
+(*   all executions of the program start by producing an expected trace *)
+(*   of I/O actions, representing the good behavior expected from the program. *)
+(*   After that, the program may terminate, or continue running, or go wrong *)
+(*   on an undefined behavior.  What matters is that the program produced *)
+(*   the expected trace at the beginning of its execution.  This is a typical *)
+(*   liveness property, and it is preserved by compilation. *) *)
 
-Definition c_program_has_initial_trace (p: ChkCsyntax.program) (t: trace): Prop :=
-  forall beh, program_behaves (ChkCsem.semantics p) beh -> behavior_prefix t beh.
-Definition asm_program_has_initial_trace (p: Asm.program) (t: trace): Prop :=
-  forall beh, program_behaves (Asm.semantics p) beh -> behavior_prefix t beh.
+(* Definition c_program_has_initial_trace (p: ChkCsyntax.program) (t: trace): Prop := *)
+(*   forall beh, program_behaves (ChkCsem.semantics p) beh -> behavior_prefix t beh. *)
+(* Definition asm_program_has_initial_trace (p: Asm.program) (t: trace): Prop := *)
+(*   forall beh, program_behaves (Asm.semantics p) beh -> behavior_prefix t beh. *)
 
-Theorem transf_c_program_preserves_initial_trace:
-  forall p tp t,
-  transf_chkc_program p = OK tp ->
-  c_program_has_initial_trace p t ->
-  asm_program_has_initial_trace tp t.
-Proof.
-  intros p tp t TRANSF CTRACE; red; intros beh AEXEC.
-  exploit transf_c_program_preservation; eauto. intros (beh' & CEXEC & IMPR).
-  apply CTRACE in CEXEC. destruct IMPR as [EQ | [t' [A B]]].
-- congruence.
-- destruct CEXEC as (beh1' & EQ').
-  destruct B as (beh1 & EQ).
-  subst beh'. destruct beh1'; simpl in A; inv A. 
-  exists (behavior_app t0 beh1). apply behavior_app_assoc.
-Qed.
+(* Theorem transf_c_program_preserves_initial_trace: *)
+(*   forall p tp t, *)
+(*   transf_chkc_program p = OK tp -> *)
+(*   c_program_has_initial_trace p t -> *)
+(*   asm_program_has_initial_trace tp t. *)
+(* Proof. *)
+(*   intros p tp t TRANSF CTRACE; red; intros beh AEXEC. *)
+(*   exploit transf_c_program_preservation; eauto. intros (beh' & CEXEC & IMPR). *)
+(*   apply CTRACE in CEXEC. destruct IMPR as [EQ | [t' [A B]]]. *)
+(* - congruence. *)
+(* - destruct CEXEC as (beh1' & EQ'). *)
+(*   destruct B as (beh1 & EQ). *)
+(*   subst beh'. destruct beh1'; simpl in A; inv A.  *)
+(*   exists (behavior_app t0 beh1). apply behavior_app_assoc. *)
+(* Qed. *)
 
-(** * Extension to separate compilation *)
+(* (** * Extension to separate compilation *) *)
 
-(** The results above were given in terms of whole-program compilation.
-    They also extend to separate compilation followed by linking. *)
+(* (** The results above were given in terms of whole-program compilation. *)
+(*     They also extend to separate compilation followed by linking. *) *)
 
-Section SEPARATE_COMPILATION.
+(* Section SEPARATE_COMPILATION. *)
 
-(** The source: a list of C compilation units *)
-Variable c_units: nlist ChkCsyntax.program.
+(* (** The source: a list of C compilation units *) *)
+(* Variable c_units: nlist ChkCsyntax.program. *)
 
-(** The compiled code: a list of Asm compilation units, obtained by separate compilation *)
-Variable asm_units: nlist Asm.program.
-Hypothesis separate_compilation_succeeds: 
-  nlist_forall2 (fun cu tcu => transf_chkc_program cu = OK tcu) c_units asm_units.
+(* (** The compiled code: a list of Asm compilation units, obtained by separate compilation *) *)
+(* Variable asm_units: nlist Asm.program. *)
+(* Hypothesis separate_compilation_succeeds:  *)
+(*   nlist_forall2 (fun cu tcu => transf_chkc_program cu = OK tcu) c_units asm_units. *)
 
-(** We assume that the source C compilation units can be linked together
-    to obtain a monolithic C program [c_program]. *)
-Variable c_program: ChkCsyntax.program.
-Hypothesis source_linking: link_list c_units = Some c_program.
+(* (** We assume that the source C compilation units can be linked together *)
+(*     to obtain a monolithic C program [c_program]. *) *)
+(* Variable c_program: ChkCsyntax.program. *)
+(* Hypothesis source_linking: link_list c_units = Some c_program. *)
 
-(** Then, linking the Asm units obtained by separate compilation succeeds. *)
-Lemma compiled_linking_succeeds:
-  { asm_program | link_list asm_units = Some asm_program }.
-Proof.
-  destruct (link_list asm_units) eqn:E. 
-- exists p; auto.
-- exfalso. 
-  exploit separate_transf_ccomp_program_correct; eauto. intros (a & P & Q).
-  congruence.
-Qed.
+(* (** Then, linking the Asm units obtained by separate compilation succeeds. *) *)
+(* Lemma compiled_linking_succeeds: *)
+(*   { asm_program | link_list asm_units = Some asm_program }. *)
+(* Proof. *)
+(*   destruct (link_list asm_units) eqn:E.  *)
+(* - exists p; auto. *)
+(* - exfalso.  *)
+(*   exploit separate_transf_ccomp_program_correct; eauto. intros (a & P & Q). *)
+(*   congruence. *)
+(* Qed. *)
 
-(** Let asm_program be the result of linking the Asm units. *)
-Let asm_program: Asm.program := proj1_sig compiled_linking_succeeds.
-Let compiled_linking: link_list asm_units = Some asm_program := proj2_sig compiled_linking_succeeds.
+(* (** Let asm_program be the result of linking the Asm units. *) *)
+(* Let asm_program: Asm.program := proj1_sig compiled_linking_succeeds. *)
+(* Let compiled_linking: link_list asm_units = Some asm_program := proj2_sig compiled_linking_succeeds. *)
 
-(** Then, [asm_program] preserves the semantics and the specifications of
-  [c_program], in the following sense.
-  First, every behavior of [asm_program] improves upon one of the possible
-  behaviors of [c_program]. *)
+(* (** Then, [asm_program] preserves the semantics and the specifications of *)
+(*   [c_program], in the following sense. *)
+(*   First, every behavior of [asm_program] improves upon one of the possible *)
+(*   behaviors of [c_program]. *) *)
 
-Theorem separate_transf_c_program_preservation:
-  forall beh,
-  program_behaves (Asm.semantics asm_program) beh ->
-  exists beh', program_behaves (ChkCsem.semantics c_program) beh' /\ behavior_improves beh' beh.
-Proof.
-  intros. exploit separate_transf_ccomp_program_correct; eauto. intros (a & P & Q).
-  assert (a = asm_program) by congruence. subst a. 
-  eapply backward_simulation_behavior_improves; eauto.
-Qed.
+(* Theorem separate_transf_c_program_preservation: *)
+(*   forall beh, *)
+(*   program_behaves (Asm.semantics asm_program) beh -> *)
+(*   exists beh', program_behaves (ChkCsem.semantics c_program) beh' /\ behavior_improves beh' beh. *)
+(* Proof. *)
+(*   intros. exploit separate_transf_ccomp_program_correct; eauto. intros (a & P & Q). *)
+(*   assert (a = asm_program) by congruence. subst a.  *)
+(*   eapply backward_simulation_behavior_improves; eauto. *)
+(* Qed. *)
 
-(** As a corollary, if [c_program] is free of undefined behaviors, 
-  the behavior of [asm_program] is one of the possible behaviors of [c_program]. *)
+(* (** As a corollary, if [c_program] is free of undefined behaviors,  *)
+(*   the behavior of [asm_program] is one of the possible behaviors of [c_program]. *) *)
 
-Theorem separate_transf_c_program_is_refinement:
-  (forall beh, program_behaves (ChkCsem.semantics c_program) beh -> not_wrong beh) ->
-  (forall beh, program_behaves (Asm.semantics asm_program) beh -> program_behaves (ChkCsem.semantics c_program) beh).
-Proof.
-  intros. exploit separate_transf_c_program_preservation; eauto. intros (beh' & P & Q).
-  assert (not_wrong beh') by auto.
-  inv Q.
-- auto.
-- destruct H2 as (t & U & V). subst beh'. elim H1. 
-Qed.
+(* Theorem separate_transf_c_program_is_refinement: *)
+(*   (forall beh, program_behaves (ChkCsem.semantics c_program) beh -> not_wrong beh) -> *)
+(*   (forall beh, program_behaves (Asm.semantics asm_program) beh -> program_behaves (ChkCsem.semantics c_program) beh). *)
+(* Proof. *)
+(*   intros. exploit separate_transf_c_program_preservation; eauto. intros (beh' & P & Q). *)
+(*   assert (not_wrong beh') by auto. *)
+(*   inv Q. *)
+(* - auto. *)
+(* - destruct H2 as (t & U & V). subst beh'. elim H1.  *)
+(* Qed. *)
 
-(** We now show that if all executions of [c_program] satisfy a specification,
-  then all executions of [asm_program] also satisfy the specification, provided
-  the specification is of the safety-enforcing kind. *)
+(* (** We now show that if all executions of [c_program] satisfy a specification, *)
+(*   then all executions of [asm_program] also satisfy the specification, provided *)
+(*   the specification is of the safety-enforcing kind. *) *)
 
-Theorem separate_transf_c_program_preserves_spec:
-  forall spec,
-  safety_enforcing_specification spec ->
-  c_program_satisfies_spec c_program spec ->
-  asm_program_satisfies_spec asm_program spec.
-Proof.
-  intros spec SES CSAT; red; intros beh AEXEC.
-  exploit separate_transf_c_program_preservation; eauto. intros (beh' & CEXEC & IMPR).
-  apply CSAT in CEXEC. destruct IMPR as [EQ | [t [A B]]].
-- congruence.
-- subst beh'. apply SES in CEXEC. contradiction. 
-Qed.
+(* Theorem separate_transf_c_program_preserves_spec: *)
+(*   forall spec, *)
+(*   safety_enforcing_specification spec -> *)
+(*   c_program_satisfies_spec c_program spec -> *)
+(*   asm_program_satisfies_spec asm_program spec. *)
+(* Proof. *)
+(*   intros spec SES CSAT; red; intros beh AEXEC. *)
+(*   exploit separate_transf_c_program_preservation; eauto. intros (beh' & CEXEC & IMPR). *)
+(*   apply CSAT in CEXEC. destruct IMPR as [EQ | [t [A B]]]. *)
+(* - congruence. *)
+(* - subst beh'. apply SES in CEXEC. contradiction.  *)
+(* Qed. *)
 
-(** As another corollary of [separate_transf_c_program_preservation],
-  if all executions of [c_program] have a trace [t] as initial trace,
-  so do all executions of [asm_program]. *)
+(* (** As another corollary of [separate_transf_c_program_preservation], *)
+(*   if all executions of [c_program] have a trace [t] as initial trace, *)
+(*   so do all executions of [asm_program]. *) *)
 
-Theorem separate_transf_c_program_preserves_initial_trace:
-  forall t,
-  c_program_has_initial_trace c_program t ->
-  asm_program_has_initial_trace asm_program t.
-Proof.
-  intros t CTRACE; red; intros beh AEXEC.
-  exploit separate_transf_c_program_preservation; eauto. intros (beh' & CEXEC & IMPR).
-  apply CTRACE in CEXEC. destruct IMPR as [EQ | [t' [A B]]].
-- congruence.
-- destruct CEXEC as (beh1' & EQ').
-  destruct B as (beh1 & EQ).
-  subst beh'. destruct beh1'; simpl in A; inv A. 
-  exists (behavior_app t0 beh1). apply behavior_app_assoc.
-Qed.
+(* Theorem separate_transf_c_program_preserves_initial_trace: *)
+(*   forall t, *)
+(*   c_program_has_initial_trace c_program t -> *)
+(*   asm_program_has_initial_trace asm_program t. *)
+(* Proof. *)
+(*   intros t CTRACE; red; intros beh AEXEC. *)
+(*   exploit separate_transf_c_program_preservation; eauto. intros (beh' & CEXEC & IMPR). *)
+(*   apply CTRACE in CEXEC. destruct IMPR as [EQ | [t' [A B]]]. *)
+(* - congruence. *)
+(* - destruct CEXEC as (beh1' & EQ'). *)
+(*   destruct B as (beh1 & EQ). *)
+(*   subst beh'. destruct beh1'; simpl in A; inv A.  *)
+(*   exists (behavior_app t0 beh1). apply behavior_app_assoc. *)
+(* Qed. *)
 
-End SEPARATE_COMPILATION.
+(* End SEPARATE_COMPILATION. *)
